Add subtyping rule [x has L:S..U => S <: U] and hmode to
control if we allow it (deeply).

Actually this is the same idea as in 0a9cf322 (exactly 11 months ago),
but this time I insisted more and it works for gDOT :-)
Note, though, that okhyp_to_nohyp currently relies on the fact that
subtyping never grows the env, which will not be the case any more
when we add existentials.

dev/existential/hmode-stable_typ-IndWf-precise-gDot.v
@@ -364,95 +364,80 @@ with wf_dec_impl: ctx -> fset typ -> dec -> Prop :=
 Notation wf_typ G T := (wf_typ_impl G \{} T).
 Notation wf_dec G D := (wf_dec_impl G \{} D).
 
-Inductive subtyp: ctx -> typ -> typ -> Prop :=
-  | subtyp_refl: forall G T,
+Inductive hmode: Set := okhyp | nohyp.
+
+Inductive subtyp: hmode -> ctx -> typ -> typ -> Prop :=
+  | subtyp_refl: forall hm G T,
       wf_typ G T ->
-      subtyp G T T
-  | subtyp_top: forall G T,
+      subtyp hm G T T
+  | subtyp_top: forall hm G T,
       wf_typ G T ->
-      subtyp G T typ_top
-  | subtyp_bot: forall G T,
+      subtyp hm G T typ_top
+  | subtyp_bot: forall hm G T,
       wf_typ G T ->
-      subtyp G typ_bot T
-  | subtyp_rcd: forall G D1 D2,
-      subdec G D1 D2 ->
-      subtyp G (typ_rcd D1) (typ_rcd D2)
-  | subtyp_sel_l: forall G x X L T U,
+      subtyp hm G typ_bot T
+  | subtyp_rcd: forall hm G D1 D2,
+      subdec hm G D1 D2 ->
+      subtyp hm G (typ_rcd D1) (typ_rcd D2)
+  | subtyp_sel_l: forall hm G x X L T U,
       binds x X G ->
       wf_typ G X ->
       stable_typ X -> (* <-- important restriction *)
       typ_has G X (dec_typ L T U) ->
-      subtyp G T U -> (* <-- probably not needed, but keep for symmetry with subtyp_sel_r *)
-      subtyp G (typ_sel (avar_f x) L) U
-  | subtyp_sel_r: forall G x X L T U,
+      subtyp hm G T U -> (* <-- probably not needed, just for symmetry with subtyp_sel_r *)
+      subtyp hm G (typ_sel (avar_f x) L) U
+  | subtyp_sel_r: forall hm G x X L T U,
       binds x X G ->
       wf_typ G X ->
       stable_typ X -> (* <-- important restriction *)
       typ_has G X (dec_typ L T U) ->
-      subtyp G T U -> (* <-- makes proofs a lot easier!! *)
-      subtyp G T (typ_sel (avar_f x) L)
-  | subtyp_and: forall G T U1 U2,
-      subtyp G T U1 ->
-      subtyp G T U2 ->
-      subtyp G T (typ_and U1 U2)
-  | subtyp_and_l: forall G T1 T2,
+      subtyp hm G T U -> (* <-- makes proofs a lot easier!! *)
+      subtyp hm G T (typ_sel (avar_f x) L)
+  | subtyp_and: forall hm G T U1 U2,
+      subtyp hm G T U1 ->
+      subtyp hm G T U2 ->
+      subtyp hm G T (typ_and U1 U2)
+  | subtyp_and_l: forall hm G T1 T2,
       wf_typ G T1 ->
       wf_typ G T2 ->
-      subtyp G (typ_and T1 T2) T1
-  | subtyp_and_r: forall G T1 T2,
+      subtyp hm G (typ_and T1 T2) T1
+  | subtyp_and_r: forall hm G T1 T2,
       wf_typ G T1 ->
       wf_typ G T2 ->
-      subtyp G (typ_and T1 T2) T2
-  | subtyp_or: forall G T1 T2 U,
-      subtyp G T1 U ->
-      subtyp G T2 U ->
-      subtyp G (typ_or T1 T2) U
-  | subtyp_or_l: forall G T1 T2,
+      subtyp hm G (typ_and T1 T2) T2
+  | subtyp_or: forall hm G T1 T2 U,
+      subtyp hm G T1 U ->
+      subtyp hm G T2 U ->
+      subtyp hm G (typ_or T1 T2) U
+  | subtyp_or_l: forall hm G T1 T2,
       wf_typ G T1 ->
       wf_typ G T2 ->
-      subtyp G T1 (typ_or T1 T2)
-  | subtyp_or_r: forall G T1 T2,
+      subtyp hm G T1 (typ_or T1 T2)
+  | subtyp_or_r: forall hm G T1 T2,
       wf_typ G T1 ->
       wf_typ G T2 ->
-      subtyp G T2 (typ_or T1 T2)
-  | subtyp_trans: forall G T1 T2 T3,
-      subtyp G T1 T2 ->
-      subtyp G T2 T3 ->
-      subtyp G T1 T3
-(* Error: Non strictly positive occurrence of "subtyp"
-   --> define the whole subtyping function as a Fixpoint with fuel?
-   --> or put the assumption in ty_trm? *)
-(*| subtyp_hyp: forall x X G L Lo Hi T1 T2,
+      subtyp hm G T2 (typ_or T1 T2)
+  | subtyp_trans: forall hm G T1 T2 T3,
+      subtyp hm G T1 T2 ->
+      subtyp hm G T2 T3 ->
+      subtyp hm G T1 T3
+  | subtyp_hyp: forall x X G L Lo Hi,
       binds x X G ->
       typ_has G X (dec_typ L Lo Hi) ->
-      (subtyp G Lo Hi -> subtyp G T1 T2) ->
-      subtyp G T1 T2
-*)
-with subdec: ctx -> dec -> dec -> Prop :=
-  | subdec_typ: forall G L Lo1 Hi1 Lo2 Hi2,
-      subtyp G Lo2 Lo1 ->
-      subtyp G Hi1 Hi2 ->
-      subdec G (dec_typ L Lo1 Hi1) (dec_typ L Lo2 Hi2)
-  | subdec_mtd: forall m G S1 T1 S2 T2,
-      subtyp G S2 S1 ->
-      subtyp G T1 T2 ->
-      subdec G (dec_mtd m S1 T1) (dec_mtd m S2 T2).
-
-Definition good_bounds_typ(G: ctx)(T: typ) :=
-  wf_typ G T /\ (forall L Lo Hi, typ_has G T (dec_typ L Lo Hi) -> subtyp G Lo Hi).
-
-Definition good_bounds(G: ctx) :=
-  forall x X, binds x X G -> good_bounds_typ G X.
-
-(*
-Inductive good_bounds: ctx -> Prop :=
-  | good_bounds_empty:
-      good_bounds empty
-  | good_bounds_push: forall G x T,
-      good_bounds G ->
-      good_bounds_typ (G & x ~ T) T ->
-      good_bounds (G & x ~ T).
-*)
+      stable_typ X ->
+      wf_typ G X ->
+      wf_typ G Lo ->
+      wf_typ G Hi ->
+      subtyp okhyp G Lo Hi
+with subdec: hmode -> ctx -> dec -> dec -> Prop :=
+  | subdec_typ: forall hm G L Lo1 Hi1 Lo2 Hi2,
+      subtyp hm G Lo2 Lo1 ->
+      subtyp hm G Hi1 Hi2 ->
+      subdec hm G (dec_typ L Lo1 Hi1) (dec_typ L Lo2 Hi2)
+  | subdec_mtd: forall hm m G S1 T1 S2 T2,
+      subtyp hm G S2 S1 ->
+      subtyp hm G T1 T2 ->
+      subdec hm G (dec_mtd m S1 T1) (dec_mtd m S2 T2).
 
 
 (* ###################################################################### *)
@@ -497,47 +482,6 @@ Inductive closed_env: ctx -> Prop :=
       closed_typ (G1 & x ~ T) T ->
       closed_env (G1 & x ~ T & G2).
 
-(*
-Inductive subenv: ctx -> ctx -> Prop :=
-(*| subenv_refl: forall G,
-      subenv G G not needed because subenv_sub with subtyp_refl yield this *)
-  | subenv_sub: forall G1 x S1 S2 G2,
-      stable_typ S1 ->
-      subtyp (G1 & x ~ S1) S1 S2 ->
-      subenv (G1 & x ~ S1 & G2) (G1 & x ~ S2 & G2)
-  | subenv_trans: forall G1 G2 G3,
-      subenv G1 G2 ->
-      subenv G2 G3 ->
-      subenv G1 G3.
-*)
-
-(* encodes any number of weakening and narrowing steps
-Inductive subenv: ctx -> ctx -> Prop :=
-  (* base case: *)
-  | subenv_empty:
-      subenv empty empty
-  (* narrowing: *)
-  | subenv_sub: forall G1 G2 x T1 T2,
-      subenv G1 G2 ->
-      stable_typ T1 ->
-      subtyp (G1 & x ~ T1) T1 T2 ->
-      subenv (G1 & x ~ T1) (G2 & x ~ T2)
-  (* not changing anything: *)
-  | subenv_push: forall G1 G2 x T,
-      (* here we don't require T to be stable *)
-      subenv G1 G2 ->
-      subenv (G1 & x ~ T) (G2 & x ~ T)
-  (* weakening: *)
-  | subenv_skip: forall G1 G2 x T,
-      subenv G1 G2 ->
-      subenv (G1 & x ~ T) G2.
-*)
-
-Definition subenv(G1 G2: ctx) :=
-  forall x T2, binds x T2 G2 -> 
-    binds x T2 G1 \/
-    exists T1, binds x T1 G1 /\ subtyp G1 T1 T2 /\ stable_typ T1.
-
 (* typing on term level is always imprecise (can use subsumption) *)
 Inductive ty_trm: ctx -> trm -> typ -> Prop :=
   | ty_var: forall G x T,
@@ -557,17 +501,10 @@ Inductive ty_trm: ctx -> trm -> typ -> Prop :=
          ty_trm (G & x ~ (open_typ x T)) (open_trm x u) U) ->
       wf_typ G U -> (* <-- even stronger than x \notin fv_typ U *)
       ty_trm G (trm_new ds u) U
-  (* If you want to suppose good bounds, you must prove the typing derivation not just
-     for G, but for all subenvs of G, because otherwise narrowing needs un-narrowing
-     and weakening needs strengthening. *)
-  | ty_hyp: forall G t T,
-      wf_typ G T ->
-      (forall G', subenv G' G -> good_bounds G' -> ty_trm G' t T) ->
-      ty_trm G t T
 (* imprecise typing: subsumption allowed *)
   | ty_sbsm: forall G t T1 T2,
       ty_trm G t T1 ->
-      subtyp G T1 T2 ->
+      subtyp okhyp G T1 T2 ->
       ty_trm G t T2
 with ty_def: ctx -> def -> dec -> Prop :=
   | ty_tdef: forall G L T,
@@ -2083,8 +2020,8 @@ Axiom okadmit: forall (G: ctx), ok G.
 
 (* If a type is involved in a subtyping judgment, it is (deeply) well-formed. *)
 Lemma subtyping_regular:
-   (forall G T1 T2, subtyp G T1 T2 -> wf_typ G T1 /\ wf_typ G T2)
-/\ (forall G D1 D2, subdec G D1 D2 -> wf_dec G D1 /\ wf_dec G D2).
+   (forall hm G T1 T2, subtyp hm G T1 T2 -> wf_typ G T1 /\ wf_typ G T2)
+/\ (forall hm G D1 D2, subdec hm G D1 D2 -> wf_dec G D1 /\ wf_dec G D2).
 Proof.
   apply subtyp_mutind; try solve [intros; split; subst; destruct_wf; eauto].
   (* case subtyp_rcd *)
@@ -2095,13 +2032,13 @@ Qed.
 Definition subtyp_regular := proj1 subtyping_regular.
 Definition subdec_regular := proj2 subtyping_regular.
 
-Definition subtyp_regular_1(G: ctx)(T1 T2: typ)(St: subtyp G T1 T2) :=
+Definition subtyp_regular_1(hm: hmode)(G: ctx)(T1 T2: typ)(St: subtyp hm G T1 T2) :=
   (proj1 (subtyp_regular St)).
-Definition subtyp_regular_2(G: ctx)(T1 T2: typ)(St: subtyp G T1 T2) :=
+Definition subtyp_regular_2(hm: hmode)(G: ctx)(T1 T2: typ)(St: subtyp hm G T1 T2) :=
   (proj2 (subtyp_regular St)).
-Definition subdec_regular_1(G: ctx)(D1 D2: dec)(Sd: subdec G D1 D2) :=
+Definition subdec_regular_1(hm: hmode)(G: ctx)(D1 D2: dec)(Sd: subdec hm G D1 D2) :=
   (proj1 (subdec_regular Sd)).
-Definition subdec_regular_2(G: ctx)(D1 D2: dec)(Sd: subdec G D1 D2) :=
+Definition subdec_regular_2(hm: hmode)(G: ctx)(D1 D2: dec)(Sd: subdec hm G D1 D2) :=
   (proj2 (subdec_regular Sd)).
 
 Hint Resolve subtyp_regular_1 subtyp_regular_2 subdec_regular_1 subdec_regular_2.
@@ -2128,6 +2065,7 @@ Proof.
   (* case ty_defs_cons *)
   introv Tyds WfT TyD WfD Hasnt.
   apply (wf_and WfT). apply wf_rcd. apply add_hyps_to_wf_dec; assumption.
+  Grab Existential Variables. constructor. constructor.
 Qed.
 
 Definition ty_trm_regular  := proj31 typing_regular.
@@ -2140,47 +2078,47 @@ Hint Resolve ty_trm_regular ty_def_regular ty_defs_regular.
 (* ###################################################################### *)
 (** ** Looks like rules, but follows from the rules *)
 
-Lemma subdec_refl: forall G D,
+Lemma subdec_refl: forall hm G D,
   wf_dec G D ->
-  subdec G D D.
+  subdec hm G D D.
 Proof.
   introv Wf. inversions Wf; eauto.
 Qed.
 
-Lemma subdec_bot: forall G D,
+Lemma subdec_bot: forall hm G D,
   wf_dec G D ->
-  subdec G (dec_bot (label_of_dec D)) D.
+  subdec hm G (dec_bot (label_of_dec D)) D.
 Proof.
   introv Wf. inversions Wf; simpl; eauto.
 Qed.
 
 Hint Resolve subdec_refl subdec_bot.
 
-Lemma subdec_intersect: forall G D0 D1 D2 D12,
-  subdec G D0 D1 ->
-  subdec G D0 D2 ->
+Lemma subdec_intersect: forall hm G D0 D1 D2 D12,
+  subdec hm G D0 D1 ->
+  subdec hm G D0 D2 ->
   D1 && D2 == D12 ->
-  subdec G D0 D12.
+  subdec hm G D0 D12.
 Proof.
   introv Sd01 Sd02 I. inversions Sd01; inversions Sd02;
   unfold intersect_dec in I; case_if; inversions I; auto.
 Qed.
 
-Lemma subdec_union: forall G D D1 D2 D12,
-  subdec G D1 D ->
-  subdec G D2 D ->
+Lemma subdec_union: forall hm G D D1 D2 D12,
+  subdec hm G D1 D ->
+  subdec hm G D2 D ->
   D1 || D2 == D12 ->
-  subdec G D12 D.
+  subdec hm G D12 D.
 Proof.
   introv Sd01 Sd02 I. inversions Sd01; inversions Sd02;
   unfold union_dec in I; case_if; inversions I; auto.
 Qed.
 
-Lemma subdec_intersect_l: forall G D1 D2 D12,
+Lemma subdec_intersect_l: forall hm G D1 D2 D12,
   D1 && D2 == D12 ->
   wf_dec G D1 ->
   wf_dec G D2 ->
-  subdec G D12 D1.
+  subdec hm G D12 D1.
 Proof.
   introv Eq WfD1 WfD2. unfold intersect_dec in Eq. case_if.
   destruct D1 as [L1 S1 U1 | m1 S1 U1];
@@ -2191,11 +2129,11 @@ Proof.
   eauto.
 Qed.
 
-Lemma subdec_intersect_r: forall G D1 D2 D12,
+Lemma subdec_intersect_r: forall hm G D1 D2 D12,
   D1 && D2 == D12 ->
   wf_dec G D1 ->
   wf_dec G D2 ->
-  subdec G D12 D2.
+  subdec hm G D12 D2.
 Proof.
   introv Eq WfD1 WfD2. unfold intersect_dec in Eq. case_if.
   destruct D1 as [L1 S1 U1 | m1 S1 U1];
@@ -2207,11 +2145,11 @@ Proof.
   eauto.
 Qed.
 
-Lemma subdec_union_l: forall G D1 D2 D12,
+Lemma subdec_union_l: forall hm G D1 D2 D12,
   D1 || D2 == D12 ->
   wf_dec G D1 ->
   wf_dec G D2 ->
-  subdec G D1 D12.
+  subdec hm G D1 D12.
 Proof.
   introv Eq Wf1 Wf2. unfold union_dec in Eq. case_if.
   destruct D1 as [L1 S1 U1 | m1 S1 U1];
@@ -2222,11 +2160,11 @@ Proof.
   eauto.
 Qed.
 
-Lemma subdec_union_r: forall G D1 D2 D12,
+Lemma subdec_union_r: forall hm G D1 D2 D12,
   D1 || D2 == D12 ->
   wf_dec G D1 ->
   wf_dec G D2 ->
-  subdec G D2 D12.
+  subdec hm G D2 D12.
 Proof.
   introv Eq Wf1 Wf2. unfold union_dec in Eq. case_if.
   destruct D1 as [L1 S1 U1 | m1 S1 U1];
@@ -2277,26 +2215,26 @@ Proof.
   inversions H; auto.
 Qed.
 
-Lemma subdec_to_label_of_dec_eq: forall G D1 D2,
-  subdec G D1 D2 -> label_of_dec D1 = label_of_dec D2.
+Lemma subdec_to_label_of_dec_eq: forall hm G D1 D2,
+  subdec hm G D1 D2 -> label_of_dec D1 = label_of_dec D2.
 Proof.
   introv Sd. inversions Sd; reflexivity.
 Qed.
 
-Lemma invert_subdec_typ_sync_left: forall G D L Lo2 Hi2,
-   subdec G D (dec_typ L Lo2 Hi2) ->
+Lemma invert_subdec_typ_sync_left: forall hm G D L Lo2 Hi2,
+   subdec hm G D (dec_typ L Lo2 Hi2) ->
    exists Lo1 Hi1, D = (dec_typ L Lo1 Hi1) /\
-                   subtyp G Lo2 Lo1 /\
-                   subtyp G Hi1 Hi2.
+                   subtyp hm G Lo2 Lo1 /\
+                   subtyp hm G Hi1 Hi2.
 Proof.
   introv Sd. inversions Sd. exists Lo1 Hi1. auto.
 Qed.
 
-Lemma invert_subdec_mtd_sync_left: forall G D m T2 U2,
-   subdec G D (dec_mtd m T2 U2) ->
+Lemma invert_subdec_mtd_sync_left: forall hm G D m T2 U2,
+   subdec hm G D (dec_mtd m T2 U2) ->
    exists T1 U1, D = (dec_mtd m T1 U1) /\
-                 subtyp G T2 T1 /\
-                 subtyp G U1 U2.
+                 subtyp hm G T2 T1 /\
+                 subtyp hm G U1 U2.
 Proof.
   introv Sd. inversions Sd. exists S1 T1. auto.
 Qed.
@@ -2313,6 +2251,7 @@ Proof.
   inversions Eq;
   inversions Wf1; inversions Wf2;
   eauto.
+  Grab Existential Variables. constructor. constructor.
 Qed.
 
 Lemma union_dec_preserves_wf: forall G D1 D2 D3,
@@ -2327,10 +2266,11 @@ Proof.
   inversions Eq;
   inversions Wf1; inversions Wf2;
   eauto.
+  Grab Existential Variables. constructor. constructor.
 Qed.
 
-Lemma subdec_trans: forall G D1 D2 D3,
-  subdec G D1 D2 -> subdec G D2 D3 -> subdec G D1 D3.
+Lemma subdec_trans: forall hm G D1 D2 D3,
+  subdec hm G D1 D2 -> subdec hm G D2 D3 -> subdec hm G D1 D3.
 Proof.
   introv H12 H23. inversions H12; inversions H23; constructor;
   solve [ assumption | (eapply subtyp_trans; eassumption)].
@@ -2611,6 +2551,7 @@ Proof.
     inversions Wf.
     - in_empty_contradiction.
     - apply (union_dec_preserves_wf H); auto.
+  Grab Existential Variables. constructor. constructor.
 Qed.
 
 Print Assumptions typ_has_preserves_wf.
@@ -2687,17 +2628,67 @@ Qed.
 
 
 (* ###################################################################### *)
+(** ** More definitions (not part of spec) *)
+
+(*
+Fixpoint power_subtyp(n0: nat)(G: ctx)(T1 T2: typ): Prop := match n0 with
+| 0 => subtyp G T1 T2
+| S n => (forall D2, typ_has G T2 D2 ->
+                     exists D1, typ_has G T1 D1 /\ power_subdec n G D1 D2)
+      /\ (power_subtyp n G T1 T2)
+end
+with power_subdec(n0: nat)(G: ctx)(D1 D2: dec): Prop :=  match n0 with
+| 0 => subdec G D1 D2
+| S n => match D1, D2 with
+  | dec_typ _ S1 U1, dec_typ _ S2 U2 => power_subtyp n G S2 S1 /\ power_subtyp n G U1 U2
+  | dec_mtd _ S1 U1, dec_mtd _ S2 U2 => power_subtyp n G S2 S1 /\ power_subtyp n G U1 U2
+  | _, _ => False
+  end
+end.
+
+(* Eval cbv in (power_subtyp 4 empty typ_bot typ_top). *)
+
+Definition memberwise_subtyp := power_subtyp 1.
+*)
+
+Definition memberwise_subtyp(G: ctx)(T1 T2: typ) := 
+  (forall D2, typ_has G T2 D2 -> exists D1, typ_has G T1 D1 /\ subdec nohyp G D1 D2)
+  /\ wf_typ G T1 /\ wf_typ G T2.
+
+(*
+Definition very_good_bounds_typ(G: ctx)(T: typ) :=
+  wf_typ G T /\
+ (forall L Lo Hi, typ_has G T (dec_typ L Lo Hi) ->
+      (* subtyp G Lo Hi /\ *) memberwise_subtyp G Lo Hi).
+
+Definition very_good_bounds(G: ctx) :=
+  forall x X, binds x X G -> very_good_bounds_typ G X.
+*)
+
+(* also power_good_bounds? *)
+
+Definition subenv(G1 G2: ctx) :=
+  forall x T2, binds x T2 G2 -> 
+    binds x T2 G1 \/
+    exists T1,
+(*    binds x T1 G1 /\ power_subtyp 2 G1 T1 T2 /\ stable_typ T1. *)
+      binds x T1 G1 /\ subtyp nohyp G1 T1 T2 /\ memberwise_subtyp G1 T1 T2 /\ stable_typ T1.
+
+
+(* ###################################################################### *)
 (** ** Weakening for subtyping *)
 
+Ltac chicken := constructor.
+
 Lemma weaken_subtyp_subdec:
-   (forall G T1 T2, subtyp G T1 T2 -> forall G1 G2 G3,
+   (forall hm G T1 T2, subtyp hm G T1 T2 -> forall G1 G2 G3,
     G = G1 & G3 ->
     ok (G1 & G2 & G3) ->
-    subtyp (G1 & G2 & G3) T1 T2)
-/\ (forall G D1 D2, subdec G D1 D2 -> forall G1 G2 G3,
+    subtyp hm (G1 & G2 & G3) T1 T2)
+/\ (forall hm G D1 D2, subdec hm G D1 D2 -> forall G1 G2 G3,
     G = G1 & G3 ->
     ok (G1 & G2 & G3) ->
-    subdec (G1 & G2 & G3) D1 D2).
+    subdec hm (G1 & G2 & G3) D1 D2).
 Proof.
   destruct weaken_has as [WHas WHasnt].
   destruct weaken_wf as [WWfTyp WWfDec].
@@ -2719,69 +2710,50 @@ Proof.
   + (* case subtyp_or_l  *) eauto.
   + (* case subtyp_or_r  *) eauto.
   + (* case subtyp_trans *) eauto.
+  + (* case subtyp_hyp   *)
+    introv Bix Has SbX WfX WfLo WfHi Eq Ok.
+    apply subtyp_hyp with x X L; ((subst; apply (binds_weaken Bix Ok)) || eauto).
   + (* case subdec_typ   *) eauto.
   + (* case subdec_mtd   *) eauto.
+  (* See
+     Zongker, D. (2006). Chicken chicken chicken: Chicken chicken.
+     Annals of Improbable Research, 12(5), 16-21.
+     https://isotropic.org/papers/chicken.pdf *)
+  Grab Existential Variables.
+  chicken.
+  chicken. chicken. chicken.
+  chicken. chicken. chicken. chicken.
 Qed.
 
-Lemma weaken_subtyp_middle: forall G1 G2 G3 S U,
+Lemma weaken_subtyp_middle: forall hm G1 G2 G3 S U,
   ok (G1 & G2 & G3) -> 
-  subtyp (G1 &     G3) S U ->
-  subtyp (G1 & G2 & G3) S U.
+  subtyp hm (G1 &     G3) S U ->
+  subtyp hm (G1 & G2 & G3) S U.
 Proof.
   introv Ok St. destruct weaken_subtyp_subdec as [P _]. apply* P.
 Qed.
 
-Lemma weaken_subtyp_end: forall G1 G2 S U,
+Lemma weaken_subtyp_end: forall hm G1 G2 S U,
   ok (G1 & G2) -> 
-  subtyp G1        S U ->
-  subtyp (G1 & G2) S U.
+  subtyp hm G1        S U ->
+  subtyp hm (G1 & G2) S U.
 Proof.
   introv Ok St. destruct weaken_subtyp_subdec as [P _].
-  specialize (P G1 S U St G1 G2 empty). repeat rewrite concat_empty_r in P. auto.
+  specialize (P _ G1 S U St G1 G2 empty). repeat rewrite concat_empty_r in P. auto.
+Qed.
+
+Lemma weaken_subdec_end: forall hm G1 G2 D1 D2,
+  ok (G1 & G2) -> 
+  subdec hm G1        D1 D2 ->
+  subdec hm (G1 & G2) D1 D2.
+Proof.
+  introv Ok St. destruct weaken_subtyp_subdec as [_ P].
+  specialize (P _ G1 D1 D2 St G1 G2 empty). repeat rewrite concat_empty_r in P. auto.
 Qed.
 
 
 (* ###################################################################### *)
-(** ** Strengthening typ_has (needed to weaken good_bounds) *)
-
-Lemma ty_defs_to_good_bounds_typ: forall G ds T,
-  ty_defs G ds T ->
-  good_bounds_typ G T.
-Proof.
-  unfold good_bounds_typ. introv Tyds. split; [eauto | idtac].
-  introv THas.
-  destruct (invert_ty_defs Tyds THas) as [d [dsHas Tyd]].
-  inversions Tyd. eauto.
-Qed.
-
-(*
-Lemma ty_defs_to_good_bounds_typ: forall G ds x T,
-  good_bounds G ->
-  ty_defs (G & x ~ T) ds T ->
-  good_bounds_typ (G & x ~ T) T.
-Proof.
-  unfold good_bounds_typ. introv Gb Tyds. split; [eauto | idtac].
-  introv THas.
-  destruct (invert_ty_defs Tyds THas) as [d [dsHas Tyd]].
-  gen_eq D: (dec_typ L Lo Hi). gen_eq G0: (G & x ~ T).
-  induction Tyd; intros Eq1 Eq2; inversions Eq2.
-  - assumption.
-  - refine (H2 _ (subenv_refl _) _ _ _ _ eq_refl eq_refl).
-Qed.
-
-Lemma ty_defs_to_good_bounds_typ: forall G ds T,
-  good_bounds G ->
-  ty_defs G ds T ->
-  good_bounds_typ G T.
-Proof.
-  unfold good_bounds_typ. introv Gb Tyds. split; [eauto | idtac].
-  introv THas.
-  destruct (invert_ty_defs Tyds THas) as [d [dsHas Tyd]].
-  gen_eq D: (dec_typ L Lo Hi). induction Tyd; intro Eq; inversions Eq.
-  - assumption.
-  - refine (H2 G (subenv_refl _) Gb Gb Tyds THas dsHas eq_refl).
-Qed.
-*)
+(** ** Strengthening typ_has (needed to weaken good_bounds and memberwise_subtyp) *)
 
 (* omg...
 
@@ -2916,6 +2888,22 @@ Proof.
   apply ((proj1 strengthen_has) _ _ _ Has G1 G2 empty eq_refl Ok Wf).
 Qed.
 
+Definition good_bounds_typ(G: ctx)(T: typ) :=
+  wf_typ G T /\ (forall L Lo Hi, typ_has G T (dec_typ L Lo Hi) -> subtyp nohyp G Lo Hi).
+
+Definition good_bounds(G: ctx) :=
+  forall x X, binds x X G -> good_bounds_typ G X.
+
+Lemma ty_defs_to_good_bounds_typ: forall G ds T,
+  ty_defs G ds T ->
+  good_bounds_typ G T.
+Proof.
+  unfold good_bounds_typ. introv Tyds. split; [eauto | idtac].
+  introv THas.
+  destruct (invert_ty_defs Tyds THas) as [d [dsHas Tyd]].
+  inversions Tyd. eauto.
+Qed.
+
 Lemma weaken_good_bounds_typ_middle: forall G1 G2 G3 T,
   ok (G1 & G2 & G3) ->
   good_bounds_typ (G1 &      G3) T ->
@@ -2940,92 +2928,35 @@ Proof.
   apply (strengthen_has_end Ok Wf Has).
 Qed.
 
-Lemma strengthen_subtyp_subdec:
-   (forall G T1 T2, subtyp G T1 T2 -> forall G1 G2 G3,
-    G = G1 & G2 & G3 ->
-    ok (G1 & G2 & G3) ->
-    wf_typ (G1 & G3) T1 ->
-    wf_typ (G1 & G3) T2 ->
-    subtyp (G1 & G3) T1 T2)
-/\ (forall G D1 D2, subdec G D1 D2 -> forall G1 G2 G3,
-    G = G1 & G2 & G3 ->
-    ok (G1 & G2 & G3) ->
-    wf_dec (G1 & G3) D1 ->
-    wf_dec (G1 & G3) D2 ->
-    subdec (G1 & G3) D1 D2).
+(*
+Lemma weaken_memberwise_subtyp_end: forall G1 G2 S U,
+  ok (G1 & G2) -> 
+  memberwise_subtyp G1        S U ->
+  memberwise_subtyp (G1 & G2) S U.
 Proof.
-  apply subtyp_mutind.
-  + (* case subtyp_refl  *) eauto.
-  + (* case subtyp_top   *) eauto.
-  + (* case subtyp_bot   *) eauto.
-  + (* case subtyp_rcd   *)
-    introv Sd IH Eq Ok Wf1 Wf2. subst.
-    apply invert_wf_rcd in Wf1.
-    apply invert_wf_rcd in Wf2.
-    eauto.
-  + (* case subtyp_sel_l *)
-    introv Bix WfX Sb XHas St IH Eq Ok Wf1 WfU. subst.
-    apply invert_wf_sel in Wf1.
-    destruct Wf1 as [X' [T' [U' [Bix' [XHas' [WfX' [WfT' WfU']]]]]]].
-    lets Eq: (strengthened_binds_unique Ok Bix Bix'). subst X'.
-    lets XHas'': ((proj1 strengthen_has) _ _ _ XHas _ _ _ eq_refl Ok WfX').
-    lets Eq: (typ_has_unique XHas' XHas'' eq_refl). inversions Eq.
-    apply (subtyp_sel_l Bix' WfX' Sb XHas').
-    apply* IH.
-  + (* case subtyp_sel_r *)
-    introv Bix WfX Sb XHas St IH Eq Ok WfT Wf1. subst.
-    apply invert_wf_sel in Wf1.
-    destruct Wf1 as [X' [T' [U' [Bix' [XHas' [WfX' [WfT' WfU']]]]]]].
-    lets Eq: (strengthened_binds_unique Ok Bix Bix'). subst X'.
-    lets XHas'': ((proj1 strengthen_has) _ _ _ XHas _ _ _ eq_refl Ok WfX').
-    lets Eq: (typ_has_unique XHas' XHas'' eq_refl). inversions Eq.
-    apply (subtyp_sel_r Bix' WfX' Sb XHas').
-    apply* IH.
-  + (* case subtyp_and   *)
-    introv St1 IH1 St2 IH2 Eq OK WfT Wf. apply invert_wf_and in Wf. destruct Wf. eauto.
-  + (* case subtyp_and_l *)
-    introv Wf1 Wf2 Eq Ok Wf Wf1'. apply invert_wf_and in Wf. destruct Wf. eauto.
-  + (* case subtyp_and_r *)
-    introv Wf1 Wf2 Eq Ok Wf Wf1'. apply invert_wf_and in Wf. destruct Wf. eauto.
-  + (* case subtyp_or    *)
-    introv St1 IH1 St2 IH2 Eq OK Wf WfU. apply invert_wf_or in Wf. destruct Wf. eauto.
-  + (* case subtyp_or_l  *)
-    introv Wf1 Wf2 Eq Ok Wf1' Wf. apply invert_wf_or in Wf. destruct Wf. eauto.
-  + (* case subtyp_or_r  *)
-    introv Wf1 Wf2 Eq Ok Wf1' Wf. apply invert_wf_or in Wf. destruct Wf. eauto.
-  + (* case subtyp_trans *)
-    (* This is very hard!!! Better don't depend on it!
-    introv St1 IH1 St2 IH2 Eq Ok Wf1 Wf3. subst.
-    lets Wf2: (proj1 (subtyp_regular St2)).
-    (* Problem: We might not be able to strengthen Wf2, i.e. wf_typ (G1 & & G3) T2 might
-       not hold.
-       But still, I believe that the conclusion always holds, but how to prove it? *)
-    apply (strengthen_subtyp_trans St1 St2 Wf1 Wf3).
-    (* probably not like this:
-    gen_eq G: (G1 & G2 & G3). gen_eq A: (@FsetImpl.empty typ).
-    induction Wf2; intros Eq1 Eq2; subst.
-    - (* case wf_top *)
-      eapply (@subtyp_trans _ _ typ_top _); eauto.
-    - (* case wf_bot *)
-      eapply (@subtyp_trans _ _ typ_bot _); eauto.
-    - (* case wf_hyp *)
-      in_empty_contradiction.
-    - (* case wf_rcd *)
-      admit. (* No chance: D might contain stuff defined only in G2! *)
-    - (* case wf_sel *)
-      specialize (IHWf2_3 Ok Wf1 Wf3). (* refine (IHWf2_3 _ _ _ _ eq_refl eq_refl). *)
-      admit.
-    - (* case wf_and *)
-      admit.
-    - (* case wf_or *)
-      admit.
-    *)
-  + (* case subdec_typ   *)
-    introv StLo IH1 StHi IH2 Eq Ok Wf1 Wf2. subst. destruct_wf. eauto.
-  + (* case subdec_mtd   *)
-    introv StLo IH1 StHi IH2 Eq Ok Wf1 Wf2. subst. destruct_wf. eauto.
+  unfold memberwise_subtyp. introv Ok MSt. simpl in *. destruct MSt as [MSt St]. split.
+  - introv UHas.
+    specialize (MSt _ (strengthen_has_end Ok (proj2 (subtyp_regular St)) UHas)).
+    destruct MSt as [D1 [SHas Sd]]. exists D1. split.
+    * apply (weaken_typ_has_end Ok SHas).
+    * apply (weaken_subdec_end Ok Sd).
+  - apply (weaken_subtyp_end Ok St).
+Qed.
 *)
-Abort. (* Don't try to prove this one! It's left here only as a memorial ;-) *)
+
+Lemma weaken_memberwise_subtyp_end: forall G1 G2 S U,
+  ok (G1 & G2) -> 
+  memberwise_subtyp G1        S U ->
+  memberwise_subtyp (G1 & G2) S U.
+Proof.
+  unfold memberwise_subtyp. introv Ok MSt. destruct MSt as [MSt [WfS WfU]]. repeat split.
+  - introv UHas. specialize (MSt _ (strengthen_has_end Ok WfU UHas)).
+    destruct MSt as [D1 [SHas Sd]]. exists D1. split.
+    * apply (weaken_typ_has_end Ok SHas).
+    * apply (weaken_subdec_end Ok Sd).
+  - apply (weaken_wf_typ_end WfS Ok).
+  - apply (weaken_wf_typ_end WfU Ok).
+Qed.
 
 
 (* ###################################################################### *)
@@ -3067,15 +2998,6 @@ Proof.
   refine (weaken_good_bounds_typ_end _ Gb).
   apply (wf_sto_to_ok_G Wf).
 Qed.
-
-(*
-Lemma wf_sto_to_good_bounds: forall s G, wf_sto s G -> good_bounds G.
-Proof.
-  introv Wf. induction Wf.
-  - apply good_bounds_empty.
-  - apply (good_bounds_push IHWf). apply (ty_defs_to_good_bounds_typ H1).
-Qed.
-*)
 
 Lemma invert_wf_sto_concat: forall s G1 G2,
   wf_sto s (G1 & G2) ->
@@ -3123,14 +3045,15 @@ Qed.
 (* ###################################################################### *)
 (** ** subtyp-and-then-lookup to lookup-and-then-subdec *)
 
-Lemma swap_sub_and_typ_has: forall G T1 T2 D2,
-  subtyp G T1 T2 ->
-  typ_has G T2 D2 ->
-  exists D1,
-    typ_has G T1 D1 /\
-    subdec G D1 D2.
+Lemma subtyp_to_memberwise: forall G T1 T2,
+  subtyp nohyp G T1 T2 ->
+  memberwise_subtyp G T1 T2.
 Proof.
-  introv St. gen D2. induction St; introv T2Has.
+  introv St. unfold memberwise_subtyp.
+  destruct (subtyp_regular St) as [Wf1 Wf2].
+  refine (conj _ (conj Wf1 Wf2)). clear Wf1 Wf2.
+  gen_eq hm: nohyp.
+  induction St; unfold memberwise_subtyp in *; introv Eq T2Has; subst.
   + (* case subtyp_refl *)
     eexists. apply (conj T2Has). apply subdec_refl.
     apply (typ_has_preserves_wf T2Has H).
@@ -3153,7 +3076,7 @@ Proof.
     rename H into Bi, H0 into Sb, H1 into WfX, H2 into XHas.
     inversions T2Has.
     lets Eq: (binds_func H1 Bi). subst T0.
-    apply IHSt. clear IHSt.
+    apply (IHSt eq_refl). clear IHSt.
     lets Eq: (typ_has_unique H3 XHas eq_refl). inversions Eq.
     exact H5.
   + (* case subtyp_and *)
@@ -3161,8 +3084,8 @@ Proof.
     - eauto.
     - eauto.
     - rename H1 into U1Has, H3 into U2Has, H5 into Eq, D1 into DU1, D0 into DU2.
-      specialize (IHSt1 _ U1Has). destruct IHSt1 as [D1 [THas Sd1]].
-      specialize (IHSt2 _ U2Has). destruct IHSt2 as [D1' [THas' Sd2]].
+      specialize (IHSt1 eq_refl _ U1Has). destruct IHSt1 as [D1 [THas Sd1]].
+      specialize (IHSt2 eq_refl _ U2Has). destruct IHSt2 as [D1' [THas' Sd2]].
       destruct (intersect_dec_label_eq _ _ Eq) as [Eq1 _].
       lets Eql1: (subdec_to_label_of_dec_eq Sd1).
       lets Eql2: (subdec_to_label_of_dec_eq Sd2).
@@ -3182,7 +3105,7 @@ Proof.
       * eauto.
       * lets WfD1: (typ_has_preserves_wf T1Has WfT1).
         lets WfD2: (typ_has_preserves_wf T2Has WfT2).
-        apply (subdec_intersect_l Eq12 WfD1 WfD2).
+        apply (subdec_intersect_l _ Eq12 WfD1 WfD2).
   + (* case subtyp_and_r *)
     rename H into WfT1, H0 into WfT2.
     lets T1Has: (typ_has_total WfT1). specialize (T1Has (label_of_dec D2)).
@@ -3196,11 +3119,11 @@ Proof.
       * eauto.
       * lets WfD1: (typ_has_preserves_wf T1Has WfT1).
         lets WfD2: (typ_has_preserves_wf T2Has WfT2).
-        apply (subdec_intersect_r Eq12 WfD1 WfD2).
+        apply (subdec_intersect_r _ Eq12 WfD1 WfD2).
   + (* case subtyp_or *)
     rename T2Has into UHas.
-    specialize (IHSt1 _ UHas). destruct IHSt1 as [D01 [T1Has Sd1]].
-    specialize (IHSt2 _ UHas). destruct IHSt2 as [D02 [T2Has Sd2]].
+    specialize (IHSt1 eq_refl _ UHas). destruct IHSt1 as [D01 [T1Has Sd1]].
+    specialize (IHSt2 eq_refl _ UHas). destruct IHSt2 as [D02 [T2Has Sd2]].
     lets Eql1: (subdec_to_label_of_dec_eq Sd1).
     lets Eql2: (subdec_to_label_of_dec_eq Sd2).
     rewrite <- Eql2 in Eql1.
@@ -3209,24 +3132,26 @@ Proof.
     - apply (subdec_union Sd1 Sd2 Eq12).
   + (* case subtyp_or_l *)
     inversions T2Has. rename H3 into T1Has, H5 into T2Has, D2 into D12, D0 into D2.
-    exists D1. apply (conj T1Has). apply (subdec_union_l H7).
+    exists D1. apply (conj T1Has). apply (subdec_union_l _ H7).
     - apply (typ_has_preserves_wf T1Has H).
     - apply (typ_has_preserves_wf T2Has H0).
   + (* case subtyp_or_r *)
     inversions T2Has. rename H3 into T1Has, H5 into T2Has, D2 into D12, D0 into D2.
-    exists D2. apply (conj T2Has). apply (subdec_union_r H7).
+    exists D2. apply (conj T2Has). apply (subdec_union_r _ H7).
     - apply (typ_has_preserves_wf T1Has H).
     - apply (typ_has_preserves_wf T2Has H0).
   + (* case subtyp_trans *)
     rename D2 into D3, T2Has into T3Has.
-    specialize (IHSt2 _ T3Has).
+    specialize (IHSt2 eq_refl _ T3Has).
     destruct IHSt2 as [D2 [T2Has Sd23]].
-    specialize (IHSt1 _ T2Has).
+    specialize (IHSt1 eq_refl _ T2Has).
     destruct IHSt1 as [D1 [T1Has Sd12]].
     exists D1. apply (conj T1Has). apply (subdec_trans Sd12 Sd23).
+  + (* case subtyp_hyp *)
+    discriminate.
 Qed.
 
-Print Assumptions swap_sub_and_typ_has.
+Print Assumptions subtyp_to_memberwise.
 
 
 (* ###################################################################### *)
@@ -3238,6 +3163,7 @@ Proof.
   intros. split; intro H0; specialize (H H0); destruct H; auto.
 Qed.
 
+(*
 Lemma supertyp_has_good_bounds: forall G T1 T2,
   subtyp G T1 T2 ->
   good_bounds_typ G T1 ->
@@ -3361,11 +3287,35 @@ Proof.
 Qed.
 
 Print Assumptions supertyp_has_good_bounds.
+*)
+
+(* ###################################################################### *)
+(** ** okhyp/nohyp *)
+
+(* the trivial direction *)
+Lemma anyhyp_to_okhyp: 
+   (forall hm G T1 T2, subtyp hm G T1 T2 -> subtyp okhyp G T1 T2)
+/\ (forall hm G D1 D2, subdec hm G D1 D2 -> subdec okhyp G D1 D2).
+Proof.
+  apply subtyp_mutind; intros; eauto.
+Qed.
+
+Definition subtyp_to_okhyp := proj1 anyhyp_to_okhyp.
+Definition subdec_to_okhyp := proj2 anyhyp_to_okhyp.
 
 
 (* ###################################################################### *)
 (** ** Narrowing on type level *)
 
+(*
+Definition subenv(G1 G2: ctx) :=
+  forall x T2, binds x T2 G2 -> 
+    binds x T2 G1 \/
+    exists T1,
+      binds x T1 G1 /\ subtyp G1 T1 T2 /\ memberwise_subtyp G1 T1 T2 /\ stable_typ T1.
+*)
+
+(*
 Lemma narrow_binds_raw: forall G1 x0 S1 S2 G2 x T2,
   binds x T2 (G1 & x0 ~ S2 & G2) ->
   subtyp (G1 & x0 ~ S1 & G2) S1 S2 ->
@@ -3449,12 +3399,16 @@ Proof.
     lets Eq: (binds_func Bi1' Bi1). subst T2.
     auto.
 Qed.
+*)
 
 Lemma narrow_binds_3: forall G1 G2 x T2,
   subenv G1 G2 ->
   ok G1 ->
   binds x T2 G2 ->
-  binds x T2 G1 \/ exists T1, binds x T1 G1 /\ subtyp G1 T1 T2 /\ stable_typ T1.
+  binds x T2 G1
+  \/ exists T1, 
+     binds x T1 G1 /\ subtyp nohyp G1 T1 T2 /\ memberwise_subtyp G1 T1 T2 /\ stable_typ T1.
+(*   binds x T1 G1 /\ power_subtyp 2 G1 T1 T2 /\ stable_typ T1. *)
 Proof.
   introv Se Ok Bi. unfold subenv in Se. apply (Se _ _ Bi).
 Qed.
@@ -3492,24 +3446,69 @@ Proof.
 Qed.
 *)
 
+Lemma memberwise_subtyp_refl: forall G T,
+  wf_typ G T ->
+  memberwise_subtyp G T T.
+Proof.
+  unfold memberwise_subtyp. introv Wf. simpl in *. refine (conj _ (conj Wf Wf)).
+  introv Has. exists D2. apply (conj Has).
+  apply subdec_refl.
+  apply (typ_has_preserves_wf Has Wf).
+Qed.
+
+(*
+Lemma power_sub_refl: forall n,
+   (forall G T, wf_typ G T -> power_subtyp n G T T)
+/\ (forall G D, wf_dec G D -> power_subdec n G D D).
+Proof.
+  intro n. induction n; split; introv Wf; simpl.
+  + apply (subtyp_refl Wf).
+  + apply (subdec_refl Wf).
+  + destruct IHn as [IH1 IH2]. refine (conj _ (IH1 _ _ Wf)).
+    introv Has. exists D2. apply (conj Has). apply IH2.
+    apply (typ_has_preserves_wf Has Wf).
+  + destruct IHn as [IH1 IH2]. inversions Wf; split; apply* IH1. 
+Qed.
+
+Definition power_subtyp_refl(n: nat) := proj1 (power_sub_refl n).
+Definition power_subdec_refl(n: nat) := proj2 (power_sub_refl n).
+
 Lemma narrow_binds_4: forall G1 G2 x T1 T2,
   wf_typ G1 T1 ->
   binds x T2 G2 ->
   binds x T1 G1 ->
   subenv G1 G2 ->
-  subtyp G1 T1 T2.
+  power_subtyp 2 G1 T1 T2.
 Proof.
   introv WfT1 Bi2 Bi1 Se.
-  lets P: (narrow_binds_3 Se (okadmit _) Bi2). destruct P as [Bi1' | [T0 [Bi1' [St Sb]]]].
-  - rewrite (binds_func Bi1' Bi1). apply (subtyp_refl WfT1).
+  lets P: (narrow_binds_3 Se (okadmit _) Bi2). 
+  destruct P as [Bi1' | [T0 [Bi1' [MSt Sb]]]].
+  - rewrite (binds_func Bi1' Bi1). apply (power_subtyp_refl _ WfT1).
   - lets Eq: (binds_func Bi1' Bi1). subst. assumption.
+Qed.
+*)
+
+Lemma narrow_binds_4: forall G1 G2 x T1 T2,
+  wf_typ G1 T1 ->
+  binds x T2 G2 ->
+  binds x T1 G1 ->
+  subenv G1 G2 ->
+  subtyp nohyp G1 T1 T2 /\ memberwise_subtyp G1 T1 T2.
+Proof.
+  introv WfT1 Bi2 Bi1 Se.
+  lets P: (narrow_binds_3 Se (okadmit _) Bi2). 
+  destruct P as [Bi1' | [T0 [Bi1' [St [MSt Sb]]]]].
+  - rewrite (binds_func Bi1' Bi1). split.
+    * apply (subtyp_refl _ WfT1).
+    * apply (memberwise_subtyp_refl WfT1).
+  - lets Eq: (binds_func Bi1' Bi1). subst. split; assumption.
 Qed.
 
 Lemma narrow_binds_5: forall G1 G2 x T2,
   wf_typ G1 T2 ->
   binds x T2 G2 ->
   subenv G1 G2 ->
-  exists T1, binds x T1 G1 /\ subtyp G1 T1 T2.
+  exists T1, binds x T1 G1 /\ subtyp nohyp G1 T1 T2.
 Proof.
   introv WfT2 Bi2 Se.
   lets P: (narrow_binds_3 Se (okadmit _) Bi2). destruct P as [Bi1' | [T0 [Bi1' [St Sb]]]].
@@ -3537,13 +3536,30 @@ Qed.
 Definition narrow_has_stable := proj1 narrow_has_hasnt_stable.
 Definition narrow_hasnt_stable := proj2 narrow_has_hasnt_stable.
 
+(* As expected, subtyp_hyp allows us to fake good bounds.
+   That's why it's better to only allow type aliases in ty_new, because otherwise
+   we would have to allow (for narrowing) and disallow (to avoid bad bounds in store)
+   the use of the subtyp_hyp rule in ty_new. 
+ 
+   Also, this means that the development could (and thus should) not use the
+   good_bounds judgment any more.
+Lemma fake_good_bounds: forall G, good_bounds G.
+Proof.
+  unfold good_bounds, good_bounds_typ.
+  introv Bi. split.
+  - admit. (* only wf-ness *)
+  - introv Has. apply (subtyp_hyp Bi Has). (* only details! *)
+Abort.
+*)
+
+(* Needed by narrow_ty *)
 Lemma narrow_has_hasnt:
    (forall G T D2, typ_has G T D2 -> forall G',
     subenv G' G ->
     wf_typ G' T -> (* G' !! *)
     exists D1,
       typ_has G' T D1 /\
-      subdec G' D1 D2)
+      subdec nohyp G' D1 D2)
 /\ (forall G T l, typ_hasnt G T l -> forall G',
     subenv G' G ->
     wf_typ G' T -> (* G' !! *)
@@ -3558,26 +3574,131 @@ Proof.
   + (* case typ_sel_has *)
     intros G x X2 L Lo2 Hi2 D2 Bix2 _ IH1 _ IH2 G' Se Wf. subst.
     apply invert_wf_sel in Wf. destruct Wf as [X1 [T [U [Bix1 [X1Has [WfX1 [WfT WfU]]]]]]].
-    lets StX: (narrow_binds_4 WfX1 Bix2 Bix1 Se).
+    destruct (narrow_binds_4 WfX1 Bix2 Bix1 Se) as [StX MStX].
     lets WfX2: (proj2 (subtyp_regular StX)).
     specialize (IH1 _ Se WfX2). destruct IH1 as [D0 [X2Has Sd0]].
     apply invert_subdec_typ_sync_left in Sd0.
     destruct Sd0 as [Lo1 [Hi1 [Eq [StLo12 StHi12]]]]. subst D0.
     lets WfHi2: (proj2 (subtyp_regular StHi12)).
     specialize (IH2 _ Se WfHi2). destruct IH2 as [D1 [Hi2Has Sd12]].
-    lets P: (swap_sub_and_typ_has StX X2Has).
+    lets P: (subtyp_to_memberwise StX). destruct P as [P _]. specialize (P _ X2Has).
             (********************)
     destruct P as [D0 [X1Has' Sd0]].
     apply invert_subdec_typ_sync_left in Sd0.
     destruct Sd0 as [Lo0 [Hi0 [Eq [StLo01 StHi01]]]]. subst D0.
     lets StLo: (subtyp_trans StLo12 StLo01).
     lets StHi: (subtyp_trans StHi01 StHi12).
-    lets P: (swap_sub_and_typ_has StHi Hi2Has).
+    lets P: (subtyp_to_memberwise StHi). destruct P as [P _]. specialize (P _ Hi2Has).
             (********************)
     destruct P as [D0 [Hi0Has Sd01]].
     exists D0. split.
     - apply (typ_sel_has Bix1 X1Has' Hi0Has).
     - apply (subdec_trans Sd01 Sd12).
+(*
+  + (* case typ_sel_has *)
+    intros G x X2 L Lo2 Hi2 D2 Bix2 _ IH1 _ IH2 G' Se Wf. subst.
+    apply invert_wf_sel in Wf. destruct Wf as [X1 [T [U [Bix1 [X1Has [WfX1 [WfT WfU]]]]]]].
+    lets N: (narrow_binds_4 WfX1 Bix2 Bix1 Se). clear N.
+    assert (P: power_subtyp 3 G' X1 X2) by admit.
+    destruct P as [P3 [P2 [P1 P0]]]. simpl in P0, P1.
+    lets WfX2: (proj2 (subtyp_regular P0)).
+    specialize (IH1 _ Se WfX2). destruct IH1 as [D0 [X2Has Sd0]].
+    apply invert_subdec_typ_sync_left in Sd0.
+    destruct Sd0 as [Lo1 [Hi1 [Eq [StLo12 StHi12]]]]. subst D0.
+    specialize (P3 _ X2Has).
+    destruct P3 as [D0 [X1Has' Sd]].
+    destruct D0 as [L' Lo0 Hi0 | ]; [idtac | (exfalso; assumption)].
+    unfold power_subdec in Sd.
+    destruct Sd as [_ [Q StHi01]].
+    lets WfHi2: (proj2 (subtyp_regular StHi12)).
+    specialize (IH2 _ Se WfHi2). destruct IH2 as [D1 [Hi2Has Sd12]].
+    (* in G', Hi2 isn't the upper bound of anything, so we cannot use Hi2Has in Q *)
+
+    specialize (P2 _ X2Has). destruct P2 as [D0 
+
+
+
+  + (* case typ_sel_has *)
+    intros G x X2 L Lo2 Hi2 D2 Bix2 _ IH1 _ IH2 G' Se Wf. subst.
+    apply invert_wf_sel in Wf. destruct Wf as [X1 [T [U [Bix1 [X1Has [WfX1 [WfT WfU]]]]]]].
+    lets N: (narrow_binds_4 WfX1 Bix2 Bix1 Se). clear N.
+    assert (P: power_subtyp 4 G' X1 X2) by admit.
+    destruct P as [P4 [P3 [P2 [P1 P0]]]]. simpl in P0, P1.
+    lets WfX2: (proj2 (subtyp_regular P0)).
+    specialize (IH1 _ Se WfX2). destruct IH1 as [D0 [X2Has Sd0]].
+    apply invert_subdec_typ_sync_left in Sd0.
+    destruct Sd0 as [Lo1 [Hi1 [Eq [StLo12 StHi12]]]]. subst D0.
+    specialize (P4 _ X2Has).
+    destruct P4 as [D0 [X1Has' Sd]].
+    destruct D0 as [L' Lo0 Hi0 | ]; [idtac | (exfalso; assumption)].
+    unfold power_subdec in Sd.
+    destruct Sd as [Q3 [Q2 [Q1 Q0]]].
+
+ fold power_subdec in Sd.
+ simpl in Sd.
+    
+    destruct Sd as [StLo01 StHi01].
+
+
+
+    (*
+    lets WfHi2: (proj2 (subtyp_regular StHi12)).
+    specialize (IH2 _ Se WfHi2). destruct IH2 as [D1 [Hi2Has Sd12]].
+    *)
+    specialize (MStX2 _ X2Has). destruct MStX2 as [D0 [X1Has' Sd]]. simpl in Sd.
+    destruct D0 as [L' Lo0 Hi0 | ]; [idtac | (exfalso; assumption)].
+    destruct Sd as [StLo01 StHi01].
+    specialize (MStX1 _+ 
+
+
+  + (* case typ_sel_has *)
+    intros G x X2 L Lo2 Hi2 D2 Bix2 _ IH1 _ IH2 G' Se Wf. subst.
+    apply invert_wf_sel in Wf. destruct Wf as [X1 [T [U [Bix1 [X1Has [WfX1 [WfT WfU]]]]]]].
+    destruct (narrow_binds_4 WfX1 Bix2 Bix1 Se) as [MStX2 [MStX1 StX]].
+    simpl in MStX1, StX.
+    lets WfX2: (proj2 (subtyp_regular StX)).
+    specialize (IH1 _ Se WfX2). destruct IH1 as [D0 [X2Has Sd0]].
+    apply invert_subdec_typ_sync_left in Sd0.
+    destruct Sd0 as [Lo1 [Hi1 [Eq [StLo12 StHi12]]]]. subst D0.
+    (*
+    lets WfHi2: (proj2 (subtyp_regular StHi12)).
+    specialize (IH2 _ Se WfHi2). destruct IH2 as [D1 [Hi2Has Sd12]].
+    *)
+    specialize (MStX2 _ X2Has). destruct MStX2 as [D0 [X1Has' Sd]]. simpl in Sd.
+    destruct D0 as [L' Lo0 Hi0 | ]; [idtac | (exfalso; assumption)].
+    destruct Sd as [StLo01 StHi01].
+    specialize (MStX1 _+ 
+
+power_subtyp
+
+  + (* case typ_sel_has *)
+    intros G x X2 L Lo2 Hi2 D2 Bix2 _ IH1 _ IH2 G' Se Wf. subst.
+    apply invert_wf_sel in Wf. destruct Wf as [X1 [T [U [Bix1 [X1Has [WfX1 [WfT WfU]]]]]]].
+    destruct (narrow_binds_4 WfX1 Bix2 Bix1 Se) as [MStX2 [MStX1 StX]].
+    simpl in MStX1, StX.
+    lets WfX2: (proj2 (subtyp_regular StX)).
+    specialize (IH1 _ Se WfX2). destruct IH1 as [D0 [X2Has Sd0]].
+    apply invert_subdec_typ_sync_left in Sd0.
+    destruct Sd0 as [Lo1 [Hi1 [Eq [StLo12 StHi12]]]]. subst D0.
+    lets WfHi2: (proj2 (subtyp_regular StHi12)).
+    specialize (IH2 _ Se WfHi2). destruct IH2 as [D1 [Hi2Has Sd12]].
+    lets P: (MStX1 _ X2Has).
+            (*****)
+    destruct P as [D0 [X1Has' Sd0]].
+    apply invert_subdec_typ_sync_left in Sd0.
+    destruct Sd0 as [Lo0 [Hi0 [Eq [StLo01 StHi01]]]]. subst D0.
+    lets StLo: (subtyp_trans StLo12 StLo01).
+    lets StHi: (subtyp_trans StHi01 StHi12).
+    lets P: (MStX2 _ X2Has).
+
+
+    lets P: (MStX2 StHi Hi2Has).
+            (********************)
+    destruct P as [D0 [Hi0Has Sd01]].
+    exists D0. split.
+    - apply (typ_sel_has Bix1 X1Has' Hi0Has).
+    - apply (subdec_trans Sd01 Sd12).
+*)
   + (* case typ_and_has_1 *)
     introv _ IH1 _ IH2. introv Se Wf. rename D into D1.
     apply invert_wf_and in Wf. destruct Wf as [Wf1 Wf2].
@@ -3598,7 +3719,7 @@ Proof.
         lets WfD1: (typ_has_preserves_wf T1Has Wf1).
         lets WfD2: (typ_has_preserves_wf T2Has Wf2).
                    (********************)
-        apply (subdec_intersect_l Eq WfD1 WfD2).
+        apply (subdec_intersect_l _ Eq WfD1 WfD2).
   + (* case typ_and_has_2 *)
     introv _ IH1 _ IH2. introv Se Wf. rename D into D1.
     apply invert_wf_and in Wf. destruct Wf as [Wf1 Wf2].
@@ -3620,7 +3741,7 @@ Proof.
         lets WfD1: (typ_has_preserves_wf T1Has Wf1).
         lets WfD2: (typ_has_preserves_wf T2Has Wf2).
                    (********************)
-        apply (subdec_intersect_r Eq WfD1 WfD2).
+        apply (subdec_intersect_r _ Eq WfD1 WfD2).
   + (* case typ_and_has_12 *)
     introv _ IH1 _ IH2 Eq. introv Se Wf. subst.
     apply invert_wf_and in Wf. destruct Wf as [Wf1 Wf2].
@@ -3638,8 +3759,8 @@ Proof.
     - lets WfD1': (proj1 (subdec_regular Sd1)).
       lets WfD2': (proj1 (subdec_regular Sd2)).
       refine (subdec_intersect _ _ Eq).
-      * refine (subdec_trans _ Sd1). apply (subdec_intersect_l Eq' WfD1' WfD2').
-      * refine (subdec_trans _ Sd2). apply (subdec_intersect_r Eq' WfD1' WfD2').
+      * refine (subdec_trans _ Sd1). apply (subdec_intersect_l _ Eq' WfD1' WfD2').
+      * refine (subdec_trans _ Sd2). apply (subdec_intersect_r _ Eq' WfD1' WfD2').
   + (* case typ_or_has *)
     introv _ IH1 _ IH2 Eq. introv Se Wf. subst.
     apply invert_wf_or in Wf. destruct Wf as [Wf1 Wf2].
@@ -3657,8 +3778,8 @@ Proof.
     - lets WfD1: (proj2 (subdec_regular Sd1)).
       lets WfD2: (proj2 (subdec_regular Sd2)).
       refine (subdec_union _ _ Eq').
-      * refine (subdec_trans Sd1 _). apply (subdec_union_l Eq WfD1 WfD2).
-      * refine (subdec_trans Sd2 _). apply (subdec_union_r Eq WfD1 WfD2).
+      * refine (subdec_trans Sd1 _). apply (subdec_union_l _ Eq WfD1 WfD2).
+      * refine (subdec_trans Sd2 _). apply (subdec_union_r _ Eq WfD1 WfD2).
   + (* case typ_top_hasnt *)
     eauto.
   + (* case typ_rcd_hasnt *)
@@ -3666,12 +3787,12 @@ Proof.
   + (* case typ_sel_hasnt *)
     intros G x X2 L Lo2 Hi2 l Bix2 X2Has' IH1 Hi2Hasnt' IH2. introv Se Wf.
     apply invert_wf_sel in Wf. destruct Wf as [X1 [T [U [Bix1 [X1Has [WfX1 [WfT WfU]]]]]]].
-    lets StX: (narrow_binds_4 WfX1 Bix2 Bix1 Se).
+    destruct (narrow_binds_4 WfX1 Bix2 Bix1 Se) as [StX MStX].
     lets WfX2: (proj2 (subtyp_regular StX)).
     specialize (IH1 _ Se WfX2). destruct IH1 as [D0 [X2Has Sd0]].
     apply invert_subdec_typ_sync_left in Sd0.
     destruct Sd0 as [Lo1 [Hi1 [Eq [StLo12 StHi12]]]]. subst D0.
-    lets P: (swap_sub_and_typ_has StX X2Has).
+    lets P: (subtyp_to_memberwise StX). destruct P as [P _]. specialize (P _ X2Has).
             (********************)
     destruct P as [D0 [X1Has' Sd0]].
     apply invert_subdec_typ_sync_left in Sd0.
@@ -3679,8 +3800,8 @@ Proof.
     lets StLo: (subtyp_trans StLo12 StLo01).
     lets StHi: (subtyp_trans StHi01 StHi12).
     destruct (subtyp_regular StHi) as [WfHi0 _].
-             (**************)
     lets P: (typ_has_total WfHi0 l). destruct P as [Hasnt | Has].
+            (*************)
     - left. apply (typ_sel_hasnt Bix1 X1Has' Hasnt).
     - right. destruct Has as [D [Eq Has]]. exists D. eauto.
   + (* case typ_and_hasnt *)
@@ -3745,6 +3866,7 @@ Proof.
       split.
       * rewrite <- Eql2. rewrite Eq1. apply Eq2.
       * apply (typ_or_has T1Has T2Has EqD).
+  Grab Existential Variables. constructor. constructor.
 Qed.
 
 Print Assumptions narrow_has_hasnt.
@@ -3771,12 +3893,12 @@ Proof.
     specialize (IHX _ Se).
     specialize (IHT _ Se).
     specialize (IHU _ Se).
-    destruct (narrow_binds_3 Se (okadmit _) Bix) as [Bix' | [X' [Bix' [St SbX']]]].
+    destruct (narrow_binds_3 Se (okadmit _) Bix) as [Bix' | [X' [Bix' [St [MSt SbX']]]]].
     - (* case "type of x remained unchanged" *)
       apply (wf_sel Bix' SbX XHas' IHX IHT IHU).
     - (* case "type of x changed from X to X'" *)
-      lets P: (swap_sub_and_typ_has St XHas'). destruct P as [D1 [S1Has Sd]].
-              (********************)
+      lets P: ((proj1 MSt) _ XHas'). destruct P as [D1 [S1Has Sd]].
+                     (***)
       apply invert_subdec_typ_sync_left in Sd. destruct Sd as [T' [U' [Eq [StT2 StU2]]]].
       subst D1.
       apply (wf_sel Bix' SbX' S1Has);
@@ -3809,14 +3931,12 @@ Qed.
 *)
 
 Lemma narrow_subtyp_subdec:
-   (forall G T1 T2, subtyp G T1 T2 -> forall G',
-    good_bounds G' ->
+   (forall hm G T1 T2, subtyp hm G T1 T2 -> forall G',
     subenv G' G ->
-    subtyp G' T1 T2)
-/\ (forall G D1 D2, subdec G D1 D2 -> forall G',
-    good_bounds G' ->
+    subtyp okhyp G' T1 T2)
+/\ (forall hm G D1 D2, subdec hm G D1 D2 -> forall G',
     subenv G' G ->
-    subdec G' D1 D2).
+    subdec okhyp G' D1 D2).
 Proof.
   apply subtyp_mutind.
   + (* case subtyp_refl *)
@@ -3828,41 +3948,43 @@ Proof.
   + (* case subtyp_rcd *)
     eauto.
   + (* case subtyp_sel_l *)
-    introv Bi2 WfX SbX XHas St IHSt. introv Gb' Se.
+    introv Bi2 WfX SbX XHas St IHSt. introv Se.
     lets WfX': (narrow_wf_typ WfX Se).
-    specialize (IHSt _ Gb' Se).
+    specialize (IHSt _ Se).
     lets XHas': (narrow_has_stable XHas SbX Se).
     lets P: (narrow_binds_3 Se (okadmit _) Bi2).
-    destruct P as [Bi1 | [X' [Bi1 [StX SbX']]]].
+    destruct P as [Bi1 | [X' [Bi1 [StX [MStX SbX']]]]].
     - (* case "type of x remained unchanged" *)
       apply (subtyp_sel_l Bi1 WfX' SbX XHas' IHSt).
     - (* case "type of x changed from X to X'" *)
-      lets P: (swap_sub_and_typ_has StX XHas'). destruct P as [D1 [X'Has Sd]].
-              (********************)
+      lets P: ((proj1 MStX) _ XHas'). destruct P as [D1 [X'Has Sd]].
+                     (****)
       apply invert_subdec_typ_sync_left in Sd. destruct Sd as [T' [U' [Eq [StT StU]]]].
       subst D1.
-      refine (subtyp_trans _ StU).
+      refine (subtyp_trans _ (subtyp_to_okhyp StU)).
       apply (subtyp_sel_l Bi1 (proj1 (subtyp_regular StX)) SbX' X'Has).
-      unfold good_bounds_typ in Gb'.
-      specialize (Gb' _ _ Bi1). destruct Gb' as [_ Gb']. apply (Gb' _ _ _ X'Has).
+      apply (subtyp_hyp Bi1 X'Has SbX' (proj1 (subtyp_regular StX))
+            (**********)               (proj2 (subtyp_regular StT))
+                                       (proj1 (subtyp_regular StU))).
   + (* case subtyp_sel_r *)
-    introv Bi2 WfX SbX XHas St IHSt. introv Gb' Se.
+    introv Bi2 WfX SbX XHas St IHSt. introv Se.
     lets WfX': (narrow_wf_typ WfX Se).
-    specialize (IHSt _ Gb' Se).
+    specialize (IHSt _ Se).
     lets XHas': (narrow_has_stable XHas SbX Se).
     lets P: (narrow_binds_3 Se (okadmit _) Bi2).
-    destruct P as [Bi1 | [X' [Bi1 [StX SbX']]]].
+    destruct P as [Bi1 | [X' [Bi1 [StX [MStX SbX']]]]].
     - (* case "type of x remained unchanged" *)
       apply (subtyp_sel_r Bi1 WfX' SbX XHas' IHSt).
     - (* case "type of x changed from X to X'" *)
-      lets P: (swap_sub_and_typ_has StX XHas'). destruct P as [D1 [X'Has Sd]].
-              (********************)
+      lets P: ((proj1 MStX) _ XHas'). destruct P as [D1 [X'Has Sd]].
+                     (****)
       apply invert_subdec_typ_sync_left in Sd. destruct Sd as [T' [U' [Eq [StT StU]]]].
       subst D1.
-      refine (subtyp_trans StT _).
+      refine (subtyp_trans (subtyp_to_okhyp StT) _).
       apply (subtyp_sel_r Bi1 (proj1 (subtyp_regular StX)) SbX' X'Has).
-      unfold good_bounds_typ in Gb'.
-      specialize (Gb' _ _ Bi1). destruct Gb' as [_ Gb']. apply (Gb' _ _ _ X'Has).
+      apply (subtyp_hyp Bi1 X'Has SbX' (proj1 (subtyp_regular StX))
+            (**********)               (proj2 (subtyp_regular StT))
+                                       (proj1 (subtyp_regular StU))).
   + (* case subtyp_and *) eauto.
   + (* case subtyp_and_l *)
     intros. subst. apply subtyp_and_l; apply* narrow_wf.
@@ -3875,6 +3997,24 @@ Proof.
     intros. subst. apply subtyp_or_r; apply* narrow_wf.
   + (* case subtyp_trans *)
     intros. apply subtyp_trans with T2; eauto.
+  + (* case subtyp_hyp *)
+    introv Bi2 XHas SbX WfX WfLo WfHi Se.
+    lets WfX': (narrow_wf_typ WfX Se).
+    lets XHas': (narrow_has_stable XHas SbX Se).
+    lets P: (narrow_binds_3 Se (okadmit _) Bi2).
+    destruct P as [Bi1 | [X' [Bi1 [StX [MStX SbX']]]]].
+    - (* case "type of x remained unchanged" *)
+      apply (subtyp_hyp Bi1 XHas' SbX WfX' (narrow_wf_typ WfLo Se) (narrow_wf_typ WfHi Se)).
+    - (* case "type of x changed from X to X'" *)
+      lets P: ((proj1 MStX) _ XHas'). destruct P as [D1 [X'Has Sd]].
+                     (****)
+      apply invert_subdec_typ_sync_left in Sd. destruct Sd as [T' [U' [Eq [StT StU]]]].
+      subst D1.
+      refine (subtyp_trans (subtyp_to_okhyp StT) _).
+      refine (subtyp_trans _ (subtyp_to_okhyp StU)).
+      lets WfX'': (proj1 (subtyp_regular StX)).
+      lets WfD: (typ_has_preserves_wf X'Has WfX''). inversions WfD.
+      apply (subtyp_hyp Bi1 X'Has SbX'); assumption.
   + (* case subdec_typ *) eauto.
   + (* case subdec_mtd *) eauto.
 Qed.
@@ -3883,6 +4023,18 @@ Print Assumptions narrow_subtyp_subdec.
 
 Definition narrow_subtyp := proj1 narrow_subtyp_subdec.
 Definition narrow_subdec := proj2 narrow_subtyp_subdec.
+
+(*
+Lemma narrow_memberwise_subtyp: forall G G' T1 T2,
+  memberwise_subtyp G T1 T2 ->
+  good_bounds G' ->
+  subenv G' G ->
+  memberwise_subtyp G' T1 T2.
+Proof.
+  unfold memberwise_subtyp. introv MSt Gb Se. repeat split.
+  - introv T2Has. (* Oh no! This needs un-narrowing for typ_has! *)
+Abort.
+*)
 
 
 (* ###################################################################### *)
@@ -3905,14 +4057,15 @@ Proof.
 Qed.
 
 Lemma subenv_trans: forall G1 G2 G3,
-  good_bounds G1 ->
   subenv G1 G2 ->
   subenv G2 G3 ->
   subenv G1 G3.
 Proof.
+Abort.
+(* Does not hold because narrow_memberwise_subtyp does not hold!
   introv Gb Se12 Se23. intros x T3 Bi3.
-  destruct (Se23 _ _ Bi3) as [Bi2 | [T2 [Bi2 [St23 Sb2]]]];
-  destruct (Se12 _ _ Bi2) as [Bi1 | [T1 [Bi1 [St12 Sb1]]]].
+  destruct (Se23 _ _ Bi3) as [Bi2 | [T2 [Bi2 [St23 [MSt23 Sb2]]]]];
+  destruct (Se12 _ _ Bi2) as [Bi1 | [T1 [Bi1 [St12 [MSt12 Sb1]]]]].
   + left. exact Bi1.
   + right. exists T1. auto.
   + right. exists T2. repeat split; try assumption.
@@ -3923,20 +4076,25 @@ Proof.
     apply (narrow_subtyp St23 Gb Se12).
           (*************)    (**)
 Qed.
+*)
 
 Lemma subenv_sub: forall G1 G2 x T1 T2,
   subenv G1 G2 ->
   stable_typ T1 ->
-  subtyp (G1 & x ~ T1) T1 T2 ->
+  subtyp nohyp (G1 & x ~ T1) T1 T2 ->
+  memberwise_subtyp (G1 & x ~ T1) T1 T2 ->
   subenv (G1 & x ~ T1) (G2 & x ~ T2).
 Proof.
-  introv Se Sb St. unfold subenv in *. intros v V Bi.
+  introv Se Sb MSt St. unfold subenv in *. intros v V Bi.
   apply binds_push_inv in Bi. destruct Bi as [[? ?] | [Ne Bi]].
   - subst. right. exists T1. auto.
   - specialize (Se _ _ Bi). destruct Se as [Bi' | Se].
     * left. auto.
-    * right. destruct Se as [V' [Bi' [StV Sb']]]. exists V'.
-      repeat split; auto. apply (weaken_subtyp_end (okadmit _) StV).
+    * right. destruct Se as [V' [Bi' [StV [MStV Sb']]]]. exists V'.
+      refine (conj _ (conj _ (conj _ Sb'))).
+      + auto.
+      + apply (weaken_subtyp_end (okadmit _) StV).
+      + apply (weaken_memberwise_subtyp_end (okadmit _) MStV).
 Qed.
 
 Lemma subenv_push: forall G1 G2 x T,
@@ -3948,8 +4106,11 @@ Proof.
   - subst. auto.
   - specialize (Se _ _ Bi). destruct Se as [Bi' | Se].
     * left. auto.
-    * right. destruct Se as [V' [Bi' [StV Sb']]]. exists V'.
-      repeat split; auto. apply (weaken_subtyp_end (okadmit _) StV).
+    * right. destruct Se as [V' [Bi' [StV [MStV Sb']]]]. exists V'.
+      refine (conj _ (conj _ (conj _ Sb'))).
+      + auto.
+      + apply (weaken_subtyp_end (okadmit _) StV).
+      + apply (weaken_memberwise_subtyp_end (okadmit _) MStV).
 Qed.
 
 Lemma subenv_skip: forall G1 G2 x T,
@@ -3960,8 +4121,11 @@ Proof.
   assert (Ne: v <> x) by admit.
   specialize (Se _ _ Bi). destruct Se as [Bi' | Se].
   * left. apply* binds_push_neq.
-  * right. destruct Se as [V' [Bi' [StV Sb']]]. exists V'.
-    repeat split; auto. apply (weaken_subtyp_end (okadmit _) StV).
+  * right. destruct Se as [V' [Bi' [StV [MStV Sb']]]]. exists V'.
+    refine (conj _ (conj _ (conj _ Sb'))).
+    + auto.
+    + apply (weaken_subtyp_end (okadmit _) StV).
+    + apply (weaken_memberwise_subtyp_end (okadmit _) MStV).
 Qed.
 
 
@@ -3988,6 +4152,7 @@ Proof.
     lets WfT': (narrow_wf_typ WfT Se).
     lets P: (narrow_binds_5 WfT' Bi2 Se). destruct P as [T1 [Bi1 St]].
     lets WfT1: (proj1 (subtyp_regular St)).
+    apply subtyp_to_okhyp in St.
     apply ty_sbsm with T1; eauto.
   + (* case ty_call *)
     introv Tyt IH1 T2Has Tyu IH2 WfV2. introv Ok Se.
@@ -3997,9 +4162,9 @@ Proof.
     lets P: (narrow_has T2Has Se (ty_trm_regular IH1)).
     destruct P as [D [T2Has' Sd]]. apply invert_subdec_mtd_sync_left in Sd.
     destruct Sd as [U2' [V2' [Eq [StU2 StV2]]]]. subst D.
-    refine (ty_sbsm _ StV2).
+    refine (ty_sbsm _ (subtyp_to_okhyp StV2)).
     apply (ty_call IH1 T2Has').
-    - apply (ty_sbsm IH2 StU2).
+    - apply (ty_sbsm IH2 (subtyp_to_okhyp StU2)).
     - apply (proj1 (subtyp_regular StV2)).
   + (* case ty_new *)
     introv Tyds IH1 Tyu IH2 WfU Ok1 Se. subst.
@@ -4007,23 +4172,11 @@ Proof.
     - apply (IH1 y yL (G' & y ~ open_typ y T) (okadmit _) (subenv_push Se)).
     - apply (IH2 y yL (G' & y ~ open_typ y T) (okadmit _) (subenv_push Se)).
     - apply* narrow_wf_typ.
-  + (* case ty_hyp *)
-    introv WfT Ty IH Ok Se. subst.
-    assert (WfT': wf_typ G' T) by apply* narrow_wf_typ.
-    apply (ty_hyp WfT').
-    intros G'' Se' Gb''.
-    (* Note that we do not have to un-narrow Gb'' to Gb', because ty_hyp now is stronger *)
-    refine (IH G'' _ Gb'' G'' (okadmit _) _).
-    - apply (subenv_trans Gb'' Se' Se).
-    - apply subenv_refl.
   + (* case ty_sbsm *)
     introv Ty IH St Ok Se. subst.
-    apply ty_hyp.
-    - lets WfT: (proj2 (subtyp_regular St)). apply* narrow_wf_typ.
-    - intros G'' Se' Gb. lets Se2: (subenv_trans Gb Se' Se).
-      apply ty_sbsm with T1.
-      * apply* IH. apply okadmit.
-      * apply* narrow_subtyp.
+    apply ty_sbsm with T1.
+    * apply* IH.
+    * apply* narrow_subtyp.
   + (* case ty_tdef *)
     introv St Ok Se. subst.
     apply ty_tdef. apply* narrow_wf.
@@ -4045,12 +4198,13 @@ Lemma narrow_ty_end: forall G x S1 S2 t T,
   ty_trm (G & x ~ S2) t T ->
   ok (G & x ~ S1) ->
   stable_typ S1 ->
-  subtyp (G & x ~ S1) S1 S2 ->
+  subtyp nohyp (G & x ~ S1) S1 S2 ->
   ty_trm (G & x ~ S1) t T.
 Proof.
   introv Ty Ok Sb St. destruct narrow_ty as [P _].
   refine (P _ _ _ Ty (G & x ~ S1) Ok _).
   apply (subenv_sub (@subenv_refl G) Sb St).
+  apply (subtyp_to_memberwise St).
 Qed.
 
 Print Assumptions narrow_ty_end.
@@ -4303,16 +4457,16 @@ Qed.
 Hint Resolve subst_has subst_hasnt subst_wf_typ subst_wf_dec.
 
 Lemma subst_subtyp_subdec: forall y S,
-   (forall G T1 T2, subtyp G T1 T2 -> forall G1 G2 x,
+   (forall hm G T1 T2, subtyp hm G T1 T2 -> forall G1 G2 x,
     G = G1 & x ~ S & G2  ->
     ok (G1 & x ~ S & G2) ->
     binds y S (G1 & G2) ->
-    subtyp (subst_ctx x y (G1 & G2)) (subst_typ x y T1) (subst_typ x y T2))
-/\ (forall G D1 D2, subdec G D1 D2 -> forall G1 G2 x,
+    subtyp hm (subst_ctx x y (G1 & G2)) (subst_typ x y T1) (subst_typ x y T2))
+/\ (forall hm G D1 D2, subdec hm G D1 D2 -> forall G1 G2 x,
     G = G1 & x ~ S & G2  ->
     ok (G1 & x ~ S & G2) ->
     binds y S (G1 & G2) ->
-    subdec (subst_ctx x y (G1 & G2)) (subst_dec x y D1) (subst_dec x y D2)).
+    subdec hm (subst_ctx x y (G1 & G2)) (subst_dec x y D1) (subst_dec x y D2)).
 Proof.
   intros y S. apply subtyp_mutind.
   + (* case subtyp_refl *)
@@ -4365,499 +4519,49 @@ Proof.
     specialize (IH12 Ok Biy).
     specialize (IH23 Ok Biy).
     apply subtyp_trans with (subst_typ x y T2); eauto.
+  + (* case subtyp_hyp *)
+    introv Bix XHas Sb WfX WfLo WfHi Eq Ok Biy. subst.
+    lets Bix': (subst_binds Bix Ok Biy).
+    apply subtyp_hyp with (subst_fvar x0 y x) (subst_typ x0 y X) L.
+    * apply Bix'.
+    * apply (subst_has XHas Ok Biy).
+    * apply (subst_stable_typ _ _ Sb).
+    * eauto.
+    * eauto.
+    * eauto.
   + (* case subdec_typ *)
     intros. subst. eq_specialize. apply subdec_typ; eauto.
   + (* case subdec_mtd *)
     intros. subst. eq_specialize. apply subdec_mtd; eauto.
+  Grab Existential Variables.
+  chicken. chicken. chicken.
+  chicken. chicken. chicken. chicken. chicken.
+  chicken. chicken.
+  chicken. chicken. chicken.
 Qed.
 
 Print Assumptions subst_subtyp_subdec.
 
-Lemma subst_subtyp: forall G1 x y S G2 T1 T2,
-  subtyp (G1 & x ~ S & G2) T1 T2 ->
+Lemma subst_subtyp: forall hm G1 x y S G2 T1 T2,
+  subtyp hm (G1 & x ~ S & G2) T1 T2 ->
   ok (G1 & x ~ S & G2) ->
   binds y S (G1 & G2) ->
-  subtyp (subst_ctx x y (G1 & G2)) (subst_typ x y T1) (subst_typ x y T2).
+  subtyp hm (subst_ctx x y (G1 & G2)) (subst_typ x y T1) (subst_typ x y T2).
 Proof.
   intros. apply* subst_subtyp_subdec.
 Qed.
 
-Lemma subtyp_subst_principle: forall G x y S T1 T2,
-  subtyp (G & x ~ S) T1 T2 ->
+Lemma subtyp_subst_principle: forall hm G x y S T1 T2,
+  subtyp hm (G & x ~ S) T1 T2 ->
   ok (G & x ~ S) ->
   binds y S G ->
-  subtyp (subst_ctx x y G) (subst_typ x y T1) (subst_typ x y T2).
+  subtyp hm (subst_ctx x y G) (subst_typ x y T1) (subst_typ x y T2).
 Proof.
   introv St Ok Biy.
   destruct (subst_subtyp_subdec y S) as [P _].
-  specialize (P _ _ _ St G empty x). repeat rewrite concat_empty_r in P.
+  specialize (P _ _ _ _ St G empty x). repeat rewrite concat_empty_r in P.
   apply (P eq_refl Ok Biy).
 Qed.
-
-Lemma subenv_binds: forall G1 G2 x S2,
-  subenv G1 G2 ->
-  binds x S2 G2 ->
-  exists S1, binds x S1 G1 /\ subtyp G1 S1 S2. (* could even give a smaller env than G1 *)
-Admitted.
-
-(* duplicate the existing entry (y ~ S), inserting it between G1 and G2
-Lemma good_bounds_duplicate_entry: forall G1 G2 x y S,
-  good_bounds (G1 & G2) ->
-  binds y S G1 ->
-  x # G1 ->
-  x # G2 ->
-  good_bounds (G1 & x ~ S & G2).
-Admitted.
-*)
-
-(* Does not hold any more with the forall-based subenv definition:
-Axiom subenv_concat_inv: forall F G1 G2,
-  subenv F (G1 & G2) ->
-  exists F1 F2, F = F1 & F2 /\ subenv F1 G1.
-*)
-
-Axiom closed_env_stuff: forall (P: Prop), P.
-
-Lemma subenv_undo_subst: forall G1' G2' G1 x y S' S G2,
-  binds y S' (G1' & G2') ->
-  binds y (subst_typ x y S) (subst_ctx x y G1 & subst_ctx x y G2) ->
-  subenv G1' (subst_ctx x y G1) ->
-  subenv (G1' & G2') (subst_ctx x y G1 & subst_ctx x y G2) ->
-  subenv (subst_ctx y x G1' & x ~ subst_typ y x S' & subst_ctx y x G2') (G1 & x ~ S & G2).
-Admitted.
-
-Lemma map_compose: forall (A B C: Type) (E: env A) (f: A -> B) (g: B -> C),
-  map g (map f E) = map (fun a => g (f a)) E.
-Admitted.
-
-Lemma map_id: forall (A: Type) (E: env A) (f: A -> A),
-  (forall x a, binds x a E -> f a = a) ->
-  map f E = E.
-Admitted.
-
-Lemma invert_fv_ctx: forall G y z Z,
-  y \notin fv_ctx_types G ->
-  binds z Z G ->
-  y \notin fv_typ Z.
-Admitted.
-
-Lemma undo_subst_ctx: forall x y G,
-  y \notin fv_ctx_types G -> subst_ctx y x (subst_ctx x y G) = G.
-Proof.
-  intros. unfold subst_ctx.
-  rewrite map_compose. apply map_id.
-  intros z Z Bi.
-  apply subst_typ_undo.
-  apply (invert_fv_ctx H Bi).
-Qed.
-
-Lemma subst_ctx_concat: forall x y G1 G2,
-   subst_ctx x y (G1 & G2) = (subst_ctx x y G1) & (subst_ctx x y G2).
-Proof.
-  intros. unfold subst_ctx. apply map_concat.
-Qed.
-
-(*
-Lemma good_bounds_insert: forall G1 x S G2,
-  good_bounds (G1 & G2) ->
-  good_bounds_typ (G1 & G2) S ->
-  good_bounds (G1 & x ~ S & G2).
-Proof.
-  introv Gb GbS. unfold good_bounds in *. intros z Z Biz.
-  apply binds_middle_inv in Biz. destruct Biz as [Biz | [[zG2 [? ?]] | [zG2 [Ne Biz]]]].
-  - apply (weaken_good_bounds_typ_middle (okadmit _)).
-    apply (Gb _ _ (binds_concat_right _ Biz)).
-  - subst. apply (weaken_good_bounds_typ_middle (okadmit _)). exact GbS.
-  - apply (weaken_good_bounds_typ_middle (okadmit _)).
-    apply (Gb _ _ (binds_concat_left Biz zG2)).
-Qed.
-*)
-
-Definition notin_ctx(x: var)(G: ctx) := x \notin (dom G) /\ x \notin (fv_ctx_types G).
-
-Lemma typ_bot_has_dec_typ: forall G L,
-  typ_has G typ_bot (dec_typ L typ_top typ_bot).
-Proof.
-  intros.
-  assert (Eq: (dec_bot (label_typ L)) = (dec_typ L typ_top typ_bot)) by reflexivity.
-  rewrite <- Eq. apply typ_bot_has.
-Qed.
-
-Lemma typ_bot_has_dec_mtd: forall G m,
-  typ_has G typ_bot (dec_mtd m typ_top typ_bot).
-Proof.
-  intros.
-  assert (Eq: (dec_bot (label_mtd m)) = (dec_mtd m typ_top typ_bot)) by reflexivity.
-  rewrite <- Eq. apply typ_bot_has.
-Qed.
-
-Lemma subst_avar_injective: forall a1 a2 x y,
-  y \notin fv_avar a1 ->
-  y \notin fv_avar a2 ->
-  subst_avar x y a1 = subst_avar x y a2 ->
-  a1 = a2.
-Proof.
-  intros.
-  destruct a1; destruct a2; simpl in *;
-  repeat rewrite if_hoist in H1; inversions* H1.
-  f_equal. apply notin_singleton in H. apply notin_singleton in H0.
-  do 2 case_var*.
-Qed.
-
-Hint Resolve subst_avar_injective.
-
-Lemma subst_typ_dec_injective:
-   (forall T1 T2 x y, y \notin fv_typ T1 -> y \notin fv_typ T2 ->
-                      subst_typ x y T1 = subst_typ x y T2 -> T1 = T2)
-/\ (forall D1 D2 x y, y \notin fv_dec D1 -> y \notin fv_dec D2 ->
-                      subst_dec x y D1 = subst_dec x y D2 -> D1 = D2).
-Proof.
-  apply typ_mutind; intros; (destruct T2 || destruct D2);
-  match goal with
-  | H: subst_typ _ _ _ = subst_typ _ _ _ |- _ => inversions H
-  | H: subst_dec _ _ _ = subst_dec _ _ _ |- _ => inversions H
-  end;
-  simpl in *; f_equal;
-  repeat match goal with
-  | H: _ \notin (_ \u _) |- _ => rewrite notin_union in H; destruct H
-  end;
-  eauto.
-Qed.
-
-Definition subst_typ_injective := proj1 subst_typ_dec_injective.
-Definition subst_dec_injective := proj2 subst_typ_dec_injective.
-
-Lemma subst_typ_notin: forall x y T, x <> y -> x \notin fv_typ (subst_typ x y T).
-Admitted.
-
-Lemma undo_subst_binds00: forall G1 x y S G2 z T,
-  y \notin fv_typ T ->
-  binds y S (G1 & G2) ->
-  notin_ctx x (G1 & G2) ->
-  binds (subst_fvar x y z) (subst_typ x y T) (G1 & G2) ->
-  binds z T (subst_ctx y x (G1 & x ~ S & G2)).
-(* Does not hold if T contains some ys, (that's why we need the first condition),
-   because (subst_ctx y x ...) removes all ys in the env! *)
-Proof.
-  introv yT Biy xG Biz.
-  unfold subst_fvar in Biz. case_var.
-  - lets Eq: (binds_func Biy Biz). subst.
-    do 2 rewrite subst_ctx_concat. unfold subst_ctx at 2. rewrite map_single.
-    rewrite (subst_typ_undo x _ yT).
-    assert (xG2: x # subst_ctx y x G2) by apply closed_env_stuff.
-    apply (binds_middle_eq _ _ xG2).
-  - rewrite <- (subst_typ_undo x _ yT). apply subst_binds_0.
-    apply (binds_weaken Biz (okadmit _)).
-Qed.
-
-(*
-Lemma subst_binds_notin: forall x y z T G,
-  x \notin fv_typ T -> (* <-- useless (always true) *)
-  binds z T (subst_ctx x y G) ->
-  binds z T G.
-Proof.
-  introv xT Biz. gen_eq G0: (subst_ctx x y G). gen G0.
-  apply (env_ind (fun G0 => binds z T G0 -> G0 = subst_ctx x y G -> binds z T G)).
-  - introv Biz Eq. exfalso. apply (binds_empty_inv Biz).
-  - rename G into G0. intros G' v V IH Biz Eq.
-    destruct (env_case G0) as [? | [v' [V' [G ?]]]].
-    * subst. unfold subst_ctx in Eq. rewrite map_empty in Eq.
-      exfalso. symmetry in Eq. apply (empty_push_inv Eq).
-    * subst. unfold subst_ctx in Eq. rewrite map_push in Eq.
-      apply eq_push_inv in Eq. destruct Eq as [? [? ?]]. subst.
-      apply binds_push_inv in Biz. destruct Biz as [[? ?] | [Ne Biz]].
-      + subst.
-    * subst v V.
-Qed.
-*)
-
-Lemma undo_binds_map: forall (A B: Type) (x: var) (v: B) (E: env A) (f: A -> B),
-  binds x v (map f E) ->
-  exists v', v = f v' /\ binds x v' E.
-Proof.
-  intros. gen E.
-  apply (env_ind (fun E => binds x v (map f E) -> exists v', v = f v' /\ binds x v' E)).
-  - intros. rewrite map_empty in H. exfalso. apply (binds_empty_inv H).
-  - introv IH H. rewrite map_push in H. apply binds_push_inv in H.
-    destruct H as [[? ?] | [Ne Bi]].
-    * subst. eauto.
-    * specialize (IH Bi). destruct IH as [v' [? IH]]. subst.
-      exists v'. auto.
-Qed.
-
-Lemma undo_map: forall (A B: Type) (E: env B) (f: A -> B),
-  exists E', map f E' = E.
-Abort.
-(* Only holds if f is surjective. *)
-
-Lemma undo_subst_binds: forall G1 x y S G2 z T,
-  binds y S (subst_ctx x y G1 & subst_ctx x y G2) ->
-  x # (G1 & G2) ->
-  binds (subst_fvar x y z) T (subst_ctx x y G1 & subst_ctx x y G2) ->
-  exists T', T = subst_typ x y T' /\ binds z T' (G1 & x ~ S & G2).
-Proof.
-  introv Biy xG Biz.
-  unfold subst_fvar in Biz. case_var.
-  - lets Eq: (binds_func Biy Biz). subst.
-    assert (xG2: x # G2) by auto.
-    exists T. split.
-    * assert (xT: x \notin fv_typ T) by apply closed_env_stuff. (* from Biz *)
-      symmetry. apply (subst_fresh_typ _ _ xT).
-    * apply (binds_middle_eq _ _ xG2).
-  - rewrite <- subst_ctx_concat in Biz. unfold subst_ctx in Biz.
-    apply undo_binds_map in Biz. destruct Biz as [T' [? Biz]].
-    exists T'. apply (conj H). apply (binds_weaken Biz (okadmit _)).
-Qed.
-
-(* Doesn't hold if the type bound for z in (G1 & x ~ S & G2) contains x
-Lemma undo_subst_binds: forall G1 x y S G2 z T,
-  x \notin fv_typ S ->
-  x \notin fv_typ T -> (* <-- useless (always true) *)
-  binds y S (subst_ctx x y G1 & subst_ctx x y G2) ->
-  x # (G1 & G2) ->
-  binds (subst_fvar x y z) T (subst_ctx x y G1 & subst_ctx x y G2) ->
-  binds z T (G1 & x ~ S & G2).
-Proof.
-  introv xS xT Biy xG Biz.
-  unfold subst_fvar in Biz. case_var.
-  - lets Eq: (binds_func Biy Biz). subst.
-    assert (xG2: x # G2) by auto.
-    apply (binds_middle_eq _ _ xG2).
-  - rewrite <- subst_ctx_concat in Biz.
-
- apply binds_concat_inv in Biz. destruct Biz as [Biz | [zG2 Biz]].
-
-rewrite <- (subst_typ_undo x _ yT). apply subst_binds_0.
-    apply (binds_weaken Biz (okadmit _)).
-Qed.
-*)
-
-Print Assumptions undo_subst_binds.
-
-(*
-Lemma undo_subst_typ_has_hasnt:
-   (forall G0 T D, typ_has G0 T D -> forall G1 x y S G2,
-    G0 = subst_ctx x y G1 & subst_ctx x y G2 ->
-    binds y S (subst_ctx x y G1 & subst_ctx x y G2) ->
-    x # G1 & G2 ->
-    exists T' D', T = subst_typ x y T' /\ D = subst_dec x y D' /\
-                  typ_has (subst_ctx y x (G1 & x ~ S & G2)) T D)
-/\ (forall G0 T l, typ_hasnt G0 T l -> forall G1 x y S G2,
-    G0 = subst_ctx x y G1 & subst_ctx x y G2 ->
-    binds y S (subst_ctx x y G1 & subst_ctx x y G2) ->
-    x # G1 & G2 ->
-    exists T', T = subst_typ x y T' /\
-               typ_hasnt (subst_ctx y x (G1 & x ~ S & G2)) T l).
-
-Lemma undo_subst_typ_has_hasnt:
-   (forall G0 T D, typ_has G0 T D -> forall G1 x y S G2,
-    G0 = subst_ctx x y G1 & subst_ctx x y G2 ->
-    binds y S (subst_ctx x y G1 & subst_ctx x y G2) ->
-    x # G1 & G2 ->
-    exists T' D', T = subst_typ x y T' /\ D = subst_dec x y D' /\
-                  typ_has (subst_ctx y x (G1 & x ~ S & G2)) T D)
-/\ (forall G0 T l, typ_hasnt G0 T l -> forall G1 x y S G2,
-    G0 = subst_ctx x y G1 & subst_ctx x y G2 ->
-    binds y S (subst_ctx x y G1 & subst_ctx x y G2) ->
-    x # G1 & G2 ->
-    exists T', T = subst_typ x y T' /\
-               typ_hasnt (subst_ctx y x (G1 & x ~ S & G2)) T l).
-Proof.
-  apply typ_has_mutind.
-  + (* case typ_bot_has *)
-    introv Eq1 Biy xG.
-    exists typ_bot (dec_bot l). destruct l; eauto.
-  + (* case typ_rcd_has *)
-    introv Eq1 Biy xG.  do 2 eexists. repeat split; auto.
-    destruct T; inversions Eq2. simpl in *.
-    apply (subst_dec_injective _ _ _ yD yT) in H0. subst.
-    apply typ_rcd_has.
-  + (* case typ_sel_has *)
-    introv Bix THas IH1 HiHas IH2. introv Eq1 Eq2 Eq3 yT yD Biy xG. subst.
-    destruct T0; inversions Eq2.
-    destruct a; inversions H0.
-    rewrite if_hoist in H1. inversions H1.
-    simpl in *.
-    assert (Eq: subst_fvar x0 y v = (If v = x0 then y else v)) by reflexivity.
-    rewrite <- Eq in Bix.
-    assert (x0T: x0 \notin fv_typ T) by apply closed_env_stuff.
-      (* because x0 is not in (G1 & G2), but T is bound in (G1 & G2) *)
-    lets EqT: (subst_typ_undo y _ x0T).
-    assert (x0Lo: x0 \notin fv_typ Lo) by apply closed_env_stuff.
-    lets EqLo: (subst_typ_undo y _ x0Lo).
-    assert (x0Hi: x0 \notin fv_typ Hi) by apply closed_env_stuff.
-    lets EqHi: (subst_typ_undo y _ x0Hi).
-    rewrite <- EqLo in *. rewrite <- EqHi in *.
-    rewrite <- EqT in Bix.
-    assert (Ne: y <> x0) by apply closed_env_stuff.
-    (* because x0 is not in (G1 & G2), but y is *)
-    assert (yFr: y \notin fv_typ (subst_typ y x0 T)) by apply (subst_typ_notin _ Ne).
-    lets P: (undo_subst_binds _ _ yFr Biy xG Bix).
-    eapply (typ_sel_has P).
-    - apply* IH1. simpl. apply notin_union. split; apply (subst_typ_notin _ Ne).
-    - apply* IH2. apply (subst_typ_notin _ Ne).
-  + (* case typ_and_has_1 *) admit.
-  + (* case typ_and_has_2 *) admit.
-  + (* case typ_and_has_12 *) admit.
-  + (* case typ_or_has *) admit.
-  + (* case typ_top_hasnt *) admit.
-  + (* case typ_rcd_hasnt *) admit.
-  + (* case typ_sel_hasnt *) admit.
-  + (* case typ_and_hasnt *) admit.
-  + (* case typ_or_hasnt_1 *) admit.
-  + (* case typ_or_hasnt_2 *) admit.
-  + (* case typ_or_hasnt_12 *) admit.
-Qed.
-
-Lemma undo_subst_typ_has_hasnt:
-   (forall G0 T0 D0, typ_has G0 T0 D0 -> forall G1 x y S G2 T D,
-    G0 = G1 & G2 ->
-    T0 = subst_typ x y T ->
-    D0 = subst_dec x y D ->
-    y \notin fv_typ T ->
-    y \notin fv_dec D ->
-    binds y S (G1 & G2) ->
-    notin_ctx x (G1 & G2) ->
-    typ_has (subst_ctx y x (G1 & x ~ S & G2)) T D)
-/\ (forall G0 T0 l, typ_hasnt G0 T0 l -> forall G1 x y S G2 T,
-    G0 = G1 & G2 ->
-    T0 = subst_typ x y T ->
-    y \notin fv_typ T ->
-    binds y S (G1 & G2) ->
-    notin_ctx x (G1 & G2) ->
-    typ_hasnt (subst_ctx y x (G1 & x ~ S & G2)) T l).
-Proof.
-  apply typ_has_mutind.
-  + (* case typ_bot_has *)
-    introv Eq1 Eq2 Eq3 yT yD Biy xG.
-    destruct T; inversions Eq2.
-    destruct l; destruct D; inversions Eq3;
-    match goal with
-    | H: typ_top = subst_typ _ _ ?T |- _ => destruct T; inversions H
-    end;
-    match goal with
-    | H: typ_bot = subst_typ _ _ ?T |- _ => destruct T; inversions H
-    end;
-    [apply typ_bot_has_dec_typ | apply typ_bot_has_dec_mtd].
-  + (* case typ_rcd_has *)
-    introv Eq1 Eq2 Eq3 yT yD Biy xG.
-    destruct T; inversions Eq2. simpl in *.
-    apply (subst_dec_injective _ _ _ yD yT) in H0. subst.
-    apply typ_rcd_has.
-  + (* case typ_sel_has *)
-    introv Bix THas IH1 HiHas IH2. introv Eq1 Eq2 Eq3 yT yD Biy xG. subst.
-    destruct T0; inversions Eq2.
-    destruct a; inversions H0.
-    rewrite if_hoist in H1. inversions H1.
-    simpl in *.
-    assert (Eq: subst_fvar x0 y v = (If v = x0 then y else v)) by reflexivity.
-    rewrite <- Eq in Bix.
-    assert (x0T: x0 \notin fv_typ T) by apply closed_env_stuff.
-      (* because x0 is not in (G1 & G2), but T is bound in (G1 & G2) *)
-    lets EqT: (subst_typ_undo y _ x0T).
-    assert (x0Lo: x0 \notin fv_typ Lo) by apply closed_env_stuff.
-    lets EqLo: (subst_typ_undo y _ x0Lo).
-    assert (x0Hi: x0 \notin fv_typ Hi) by apply closed_env_stuff.
-    lets EqHi: (subst_typ_undo y _ x0Hi).
-    rewrite <- EqLo in *. rewrite <- EqHi in *.
-    rewrite <- EqT in Bix.
-    assert (Ne: y <> x0) by apply closed_env_stuff.
-    (* because x0 is not in (G1 & G2), but y is *)
-    assert (yFr: y \notin fv_typ (subst_typ y x0 T)) by apply (subst_typ_notin _ Ne).
-    lets P: (undo_subst_binds _ _ yFr Biy xG Bix).
-    eapply (typ_sel_has P).
-    - apply* IH1. simpl. apply notin_union. split; apply (subst_typ_notin _ Ne).
-    - apply* IH2. apply (subst_typ_notin _ Ne).
-  + (* case typ_and_has_1 *) admit.
-  + (* case typ_and_has_2 *) admit.
-  + (* case typ_and_has_12 *) admit.
-  + (* case typ_or_has *) admit.
-  + (* case typ_top_hasnt *) admit.
-  + (* case typ_rcd_hasnt *) admit.
-  + (* case typ_sel_hasnt *) admit.
-  + (* case typ_and_hasnt *) admit.
-  + (* case typ_or_hasnt_1 *) admit.
-  + (* case typ_or_hasnt_2 *) admit.
-  + (* case typ_or_hasnt_12 *) admit.
-Qed.
-
-Lemma undo_subst_typ_has: forall G1 x y S G2 T D,
-  y \notin fv_typ T ->
-  y \notin fv_dec D ->
-  binds y S (G1 & G2) ->
-  notin_ctx x (G1 & G2) ->
-  typ_has (G1 & G2) (subst_typ x y T) (subst_dec x y D) ->
-  typ_has (subst_ctx y x (G1 & x ~ S & G2)) T D.
-Proof.
-  intros. destruct undo_subst_typ_has_hasnt as [P _].
-  apply (P _ _ _ H3 _ _ _ _ _ _ _ eq_refl eq_refl eq_refl H H0 H1 H2).
-Qed.
-
-Lemma undo_subst_wf_typ: forall G1 x y S G2 T,
-  y \notin fv_typ T ->
-  binds y S (G1 & G2) ->
-  notin_ctx x (G1 & G2) ->
-  wf_typ (G1 & G2) (subst_typ x y T) ->
-  wf_typ (subst_ctx y x (G1 & x ~ S & G2)) T.
-Admitted.
-
-Lemma undo_subst_subtyp: forall G1 x y S G2 T1 T2,
-(*
-  y \notin fv_typ T1 ->
-  y \notin fv_typ T2 ->
-???*)
-  binds y S (G1 & G2) ->
-  notin_ctx x (G1 & G2) ->
-  subtyp (G1 & G2) (subst_typ x y T1) (subst_typ x y T2) ->
-  subtyp (subst_ctx y x (G1 & x ~ S & G2)) T1 T2.
-Admitted.
-
-(*
-Lemma undo_subst_good_bounds_typ: forall G1 x y S G2 T,
-  binds y S (subst_ctx x y G1 & subst_ctx x y G2) ->
-  x # (G1 & G2) ->
-  good_bounds_typ (subst_ctx x y G1 & subst_ctx x y G2) T ->
-  exists T', T = subst_typ x y T' /\ good_bounds_typ (G1 & x ~ S & G2) T'.
-*)
-*)
-
-Lemma undo_subst_good_bounds_typ: forall G1 x y S G2 T,
-  binds y S (subst_ctx x y G1 & subst_ctx x y G2) ->
-  x # (G1 & G2) ->
-  good_bounds_typ (subst_ctx x y G1 & subst_ctx x y G2) (subst_typ x y T) ->
-  good_bounds_typ (G1 & x ~ S & G2) T.
-Admitted.
-
-(*
-Lemma undo_subst_good_bounds_typ: forall G1 x y S G2 T,
-  y \notin fv_typ T ->
-  binds y S (G1 & G2) ->
-  notin_ctx x (G1 & G2) ->
-  good_bounds_typ (G1 & G2) (subst_typ x y T) ->
-  good_bounds_typ (subst_ctx y x (G1 & x ~ S & G2)) T.
-Proof.
-  introv yT Biy xG Gb.
-  unfold good_bounds_typ in *.
-  split.
-  - destruct Gb as [Wf _].
-    apply (undo_subst_wf_typ _ yT Biy xG Wf).
-  - destruct Gb as [_ Gb].
-    introv THas.
-    do 2 rewrite subst_ctx_concat in THas. unfold subst_ctx in THas at 2.
-    rewrite map_single in THas.
-    lets Biy': (subst_binds_0 y x Biy). rewrite subst_ctx_concat in Biy'.
-    (* Note: THas comes from a negative position, so here we don't need to undo_subst,
-       but to subst: *)
-    lets THas': (subst_has THas (okadmit _) Biy').
-    rewrite <- subst_ctx_concat in THas'.
-    rewrite (undo_subst_ctx _ _ (proj2 xG)) in THas'. simpl in THas'.
-    specialize (Gb _ _ _ THas').
-    (*
-    refine (undo_subst_subtyp _ _ _ _ Biy xG Gb).
-    admit. admit. *)
-    refine (undo_subst_subtyp _ _ Biy xG Gb).
-Qed.
-*)
 
 Lemma invert_binds_middle: forall (A: Type) (S T: A) (G1 G2: env A) (x y: var),
   ok (G1 & x ~ S & G2) ->
@@ -4870,217 +4574,6 @@ Proof.
   - subst. right. auto.
   - left. apply (binds_concat_left Bi yG2). 
 Qed.
-
-(*
-Lemma undo_subst_good_bounds: forall G1 x y S G2 ,
-  binds y S (subst_ctx x y G1 & subst_ctx x y G2) ->
-  x # (G1 & G2) ->
-  good_bounds (subst_ctx x y G1 & subst_ctx x y G2) ->
-  good_bounds (G1 & x ~ S & G2).
-*)
-
-(* This one looks nice by itself, but if it's applied with
-   G1 := (subst_typ y x G1'), so we're again replacing too many ys, which is bad.
-   But if we apply if with G1 := G1', where G1' is chosen smartly, it might be good. *)
-Lemma undo_subst_good_bounds: forall G1 x y S G2 ,
-  binds y S (subst_ctx x y G1 & subst_ctx x y G2) ->
-  x # (G1 & G2) ->
-  good_bounds (subst_ctx x y G1 & subst_ctx x y G2) ->
-  good_bounds (G1 & x ~ S & G2).
-Proof.
-  introv Biy xG Gb.
-  unfold good_bounds in *.
-  intros z Z Biz.
-  apply (subst_binds_0 x y) in Biz.
-  do 2 rewrite subst_ctx_concat in Biz. unfold subst_ctx in Biz at 2.
-  rewrite map_single in Biz.
-  apply (invert_binds_middle (okadmit _)) in Biz. destruct Biz as [Biz | [? ?]].
-  + specialize (Gb _ _ Biz).
-    refine (undo_subst_good_bounds_typ _ Biy xG Gb).
-  + subst. specialize (Gb _ _ Biy).
-    assert (xS: x \notin fv_typ S) by apply closed_env_stuff. (* from Biy *)
-    rewrite (subst_fresh_typ _ _ xS) in H0. subst.
-    refine (undo_subst_good_bounds_typ _ Biy xG Gb).
-Qed.
-
-(*
-Lemma undo_subst_good_bounds: forall G1 x y S G2,
-  binds y S (G1 & G2) ->
-  notin_ctx x (G1 & G2) ->
-  good_bounds (G1 & G2) ->
-  exists G1' S' G2',
-    subst_ctx x y G1' = G1 /\
-    subst_typ x y S'  = S  /\
-    subst_ctx x y G2' = G2 /\
-    good_bounds (G1' & x ~ S' & G2').
-Admitted.
-
-Lemma undo_subst_good_bounds: forall G1 x y S G2,
-  binds y S (G1 & G2) ->
-  notin_ctx x (G1 & G2) ->
-  good_bounds (G1 & G2) ->
-  good_bounds (subst_ctx y x (G1 & x ~ S & G2)).
-Proof.
-  introv Biy xG Gb.
-  unfold good_bounds in *.
-  intros z Z Biz.
-  apply (subst_binds_0 x y) in Biz.
-  assert (xG': x \notin fv_ctx_types (G1 & x ~ S & G2)) by apply closed_env_stuff.
-  rewrite (undo_subst_ctx _ _ xG') in Biz.
-  apply (invert_binds_middle (okadmit _)) in Biz. destruct Biz as [Biz | [? ?]].
-  + specialize (Gb _ _ Biz).
-    refine (undo_subst_good_bounds_typ _ _ Biy xG Gb). admit. (*???*)
-  + subst. specialize (Gb _ _ Biy).
-    refine (undo_subst_good_bounds_typ _ _ Biy xG Gb). admit. (*???*)
-Qed.
-*)
-
-(*
-Lemma subst_binds_2: forall G1 x S G2 z Z y,
-  binds z Z (G1 & x ~ S & G2) ->
-  ok (G1 & x ~ S & G2) ->
-  binds y S G1 ->
-  binds (subst_fvar x y z) (subst_typ x y Z) (G1 & (subst_ctx x y G2)).
-Proof.
-  introv Biz Ok Biy. unfold subst_fvar. apply binds_middle_inv in Biz.
-  destruct Biz as [Biz | [[zG2 [? ?]] | [zG2 [Ne Biz]]]]; subst; case_if.
-  - admit. (* contradiction Ok Biz *)
-  - apply binds_concat_right. apply subst_binds_0. exact Biz.
-  - apply (binds_concat_left_ok (okadmit _)).
-    assert (Eq: (subst_typ x y S) = S) by admit. (* because x not in G1 *)
-    rewrite Eq. exact Biy.
-  - apply (binds_concat_left_ok (okadmit _)).
-    assert (Eq: (subst_typ x y Z) = Z) by admit. (* because x not in G1 *)
-    rewrite Eq. exact Biz.
-Qed.
-
-Lemma undo_subst_subenv: forall G1 G1' x y S G2 G2',
-  binds y S (G1 & G2) ->
-  x # (G1 & G2) ->
-  subenv (G1' & G2') (subst_ctx x y G1 & subst_ctx x y G2) ->
-  exists G1'' G2'',
-    subst_ctx x y G1'' = G1' /\
-    subst_ctx x y G2'' = G2' /\
-    subenv (G1'' & x ~ S & G2'') (G1 & x ~ S & G2).
-Admitted.
-
-Lemma undo_subst_subenv: forall G' G1 x y S G2,
-  binds y S (G1 & G2) ->
-  x # (G1 & G2) ->
-  subenv G' (subst_ctx x y G1 & subst_ctx x y G2) ->
-  exists G'',
-    subst_ctx x y G'' = G' /\
-    subenv G'' (G1 & x ~ S & G2).
-Admitted.
-*)
-
-Lemma undo_subst_subenv: forall G' G1 x y S G2,
-  binds y S (G1 & G2) ->
-  x # G' ->
-  subenv G' (subst_ctx x y G1 & subst_ctx x y G2) ->
-  exists G1' S' G2',
-    subst_ctx x y G1' & subst_ctx x y G2' = G' /\ (* impossible if G' already contains x! *)
-    binds y S' (G1' & G2') /\
-    subenv (G1' & x ~ S' & G2') (G1 & x ~ S & G2).
-Proof.
-  introv Biy xG' Se. (*destruct (classicT (x # G')) as [xG' | xG'].
-{*)
-  lets Biy': (subst_binds_0 x y Biy). rewrite subst_ctx_concat in Biy'.
-  assert (xS: x \notin fv_typ S) by apply closed_env_stuff.
-  rewrite (subst_fresh_typ _ _ xS) in Biy'.
-  lets P: (Se _ _ Biy'). destruct P as [Biy'' | [S' [Biy'' [St Sb]]]].
-  + exists G' S (@empty typ). unfold subst_ctx at 2. rewrite map_empty.
-    repeat rewrite concat_empty_r.
-    assert (xG'': x \notin fv_ctx_types G') by apply closed_env_stuff.
-      (* from xG' and closed env *)
-    refine (conj (subst_fresh_ctx _ _ xG'') (conj Biy'' _)).
-    unfold subenv in *.
-    intros v V Biv. apply (invert_binds_middle (okadmit _)) in Biv.
-    destruct Biv as [Biv | [? ?]].
-    - lets Biv': (subst_binds_0 x y Biv). rewrite subst_ctx_concat in Biv'.
-      assert (xV: x \notin fv_typ V) by apply closed_env_stuff.
-      rewrite (subst_fresh_typ _ _ xV) in Biv'.
-      assert (x <> v) by apply closed_env_stuff. (* x is not in G' but v is *)
-      specialize (Se _ _ Biv'). destruct Se as [Biv'' | [V' [Biv'' [StV SbV]]]].
-      * left. auto.
-      * right.
-        exists V'. repeat split; auto. apply (weaken_subtyp_end (okadmit _) StV).
-    - subst. left. auto.
-  + exists G' S' (@empty typ). unfold subst_ctx at 2. rewrite map_empty.
-    repeat rewrite concat_empty_r.
-    assert (xG'': x \notin fv_ctx_types G') by apply closed_env_stuff.
-      (* from xG' and closed env *)
-    refine (conj (subst_fresh_ctx _ _ xG'') (conj Biy'' _)).
-    unfold subenv in *.
-    intros v V Biv. apply (invert_binds_middle (okadmit _)) in Biv.
-    destruct Biv as [Biv | [? ?]].
-    - lets Biv': (subst_binds_0 x y Biv). rewrite subst_ctx_concat in Biv'.
-      assert (xV: x \notin fv_typ V) by apply closed_env_stuff.
-      rewrite (subst_fresh_typ _ _ xV) in Biv'.
-      assert (x <> v) by apply closed_env_stuff. (* x is not in G' but v is *)
-      specialize (Se _ _ Biv'). destruct Se as [Biv'' | [V' [Biv'' [StV SbV]]]].
-      * left. auto.
-      * right.
-        exists V'. repeat split; auto. apply (weaken_subtyp_end (okadmit _) StV).
-    - subst. right.
-      exists S'. repeat split; auto. apply (weaken_subtyp_end (okadmit _) St).
-(*
-} {
-  unfold notin in xG'. apply not_not_elim in xG'. (* classical logic we don't really need,
-    but it's just handy here ^^ *)
-  apply get_some in xG'. destruct xG' as [S' Bix].
-  eexists. exists S' (@empty typ). unfold subst_ctx at 2. rewrite map_empty.
-  repeat rewrite concat_empty_r.
-(*
-Problem: Given a context G', which contains a binding for x, give a context G such that
-(subst_ctx x y G) = G'.
-
-But how can this work? Note that (subst_typ x y) is not surjective:
-There are some types T (those which contain x) which have no preimage under
-(subst_typ x y).
-
-Or in other words: (subst_ctx x y ?269922) contains no xs at all in its types,
-but G' might contain some, so the equality "subst_ctx x y ?269922 = G'" cannot hold!
-*)
-}
-*)
-Qed.
-
-Lemma decide_binds: forall (A: Type) (x: var) (E: env A),
-  x # E \/ exists v, binds x v E.
-Admitted.
-
-Lemma expose_binds: forall (A: Type) (x: var) (v: A) (E: env A),
-  binds x v E ->
-  exists E1 E2, E = E1 & x ~ v & E2.
-Admitted.
-
-Lemma rename_subenv: forall G1' x y T G2' G,
-  x # G ->
-  y # (G1' & x ~ T & G2') ->
-  subenv (G1' & x ~ T & G2') G ->
-  subenv ((subst_ctx x y G1') & y ~ (subst_typ x y T) & (subst_ctx x y G2')) G.
-Admitted.
-
-Lemma rename_good_bounds: forall G1 x y T G2,
-  y # (G1 & x ~ T & G2) ->
-  good_bounds (G1 & x ~ T & G2) ->
-  good_bounds ((subst_ctx x y G1) & y ~ (subst_typ x y T) & (subst_ctx x y G2)).
-Admitted.
-
-Lemma rename_ty_trm: forall G1 x y T G2 u U,
-  y # (G1 & x ~ T & G2) ->
-  ty_trm (G1 & x ~ T & G2) u U ->
-  ty_trm ((subst_ctx x y G1) & y ~ (subst_typ x y T) & (subst_ctx x y G2))
-         (subst_trm x y u)
-         (subst_typ x y U).
-Admitted.
-
-Lemma swap_subst_ctx: forall x1 y1 x2 y2 G,
-  x1 <> y2 ->
-  x2 <> y1 ->
-  (subst_ctx x1 y1 (subst_ctx x2 y2 G)) = (subst_ctx x2 y2 (subst_ctx x1 y1 G)).
-Abort.
 
 Lemma subst_ty:
    (forall G t T, ty_trm G t T -> forall G1 x y S G2,
@@ -5139,175 +4632,6 @@ Proof.
       rewrite P in IH2. clear P.
       apply IH2. apply (binds_push_neq _ Biy). auto.
     - apply (subst_wf_typ WfU Ok Biy).
-  + (* case ty_hyp *)
-    introv WfT Ty IH Eq Ok Biy. subst.
-    apply ty_hyp.
-    - apply* subst_wf_typ.
-    - intros G' Se Gb.
-      rewrite subst_ctx_concat in *.
-      assert (xG: x # (G1 & G2)) by apply closed_env_stuff.
-      destruct (decide_binds x G') as [xG' | [X Bix]].
-      { lets P: (undo_subst_subenv Biy xG' Se).
-        destruct P as [G1' [S' [G2' [? [Biy' Se']]]]]. subst.
-        rewrite <- subst_ctx_concat.
-        refine (IH _ Se' _ _ x y _ _ eq_refl (okadmit _) Biy').
-        assert (xG'': x # G1' & G2') by apply closed_env_stuff. (* from xG' *)
-        refine (undo_subst_good_bounds _ xG'' Gb).
-        apply (subst_binds_0 x y) in Biy'.
-        assert (xS': x \notin fv_typ S') by apply closed_env_stuff.
-        rewrite (subst_fresh_typ _ _ xS') in Biy'.
-        rewrite subst_ctx_concat in Biy'.
-        exact Biy'. }
-      { (* Note: G' is a subenv of  (subst_ctx x y G1 & subst_ctx x y G2), i.e. an env
-           which does not bind x, so X can be anything completely unrelated to S. 
-           --> Idea: replace x by a completely fresh x'. *)
-        destruct (expose_binds Bix) as [G1' [G2' ?]]. subst.
-        pick_fresh x'.
-
-        (* also need to do (subst x' x ...) at the end (i.e. on the goal) *)
-        (* replace x by x' in the goal (note that (subst_trm x y t) and (subst_typ x y T)
-           remain unchanged because they don't refer to x) *)
-        assert (E: x' \notin fv_ctx_types G1') by auto.
-        rewrite <- (subst_fresh_ctx x _ E). clear E.
-        assert (E: x' \notin fv_ctx_types G2') by auto.
-        rewrite <- (subst_fresh_ctx x _ E). clear E.
-        assert (E: x' \notin fv_typ X) by auto.
-        rewrite <- (subst_fresh_typ x _ E). clear E.
-        assert (E: x' \notin fv_trm (subst_trm x y t)) by apply closed_env_stuff.
-        rewrite <- (subst_fresh_trm x _ E). clear E.
-        assert (E: x' \notin fv_typ (subst_typ x y T)) by apply closed_env_stuff.
-        rewrite <- (subst_fresh_typ x _ E). clear E.
-        assert (xG5: x # G1' & x' ~ X & G2') by apply closed_env_stuff.
-        apply (rename_ty_trm xG5).
-
-        assert (xG': x # (subst_ctx x x' G1' & x' ~ subst_typ x x' X & subst_ctx x x' G2'))
-          by apply closed_env_stuff.
-        assert (x'G': x' # (G1' & x ~ X & G2')) by auto.
-        assert (xG2: x # (subst_ctx x y G1 & subst_ctx x y G2)) by apply closed_env_stuff.
-        lets Se': (rename_subenv xG2 x'G' Se).
-        lets P: (undo_subst_subenv Biy xG' Se').
-        destruct P as [G1'' [S'' [G2'' [Eq [Biy'' Se'']]]]].
-        specialize (IH _ Se'').
-
-        (* We need a goal of the form "ty_trm (subst_ctx x y ...) ... ..." to apply IH,
-           and Eq should help us to achieve this... *)
-        assert (Eq': subst_ctx x' x (subst_ctx x y G1'' & subst_ctx x y G2'')
-                   = G1' & x' ~ X & G2'). {
-          lets Eq': (f_equal (subst_ctx x' x) Eq).
-          assert (Eq2: subst_ctx x' x
-                        (subst_ctx x x' G1' & x' ~ subst_typ x x' X & subst_ctx x x' G2')
-                   = G1' & x' ~ X & G2'). {
-            do 2 rewrite subst_ctx_concat. unfold subst_ctx at 3. rewrite map_single.
-            assert (E: x' \notin fv_ctx_types G1') by auto.
-            rewrite (undo_subst_ctx x _ E). clear E.
-            assert (E: x' \notin fv_ctx_types G2') by auto.
-            rewrite (undo_subst_ctx x _ E). clear E.
-            assert (E: x' \notin fv_typ X) by auto.
-            rewrite (subst_typ_undo x _ E). clear E.
-            reflexivity.
-          }
-          rewrite Eq2 in Eq'.
-          (*rewrite <- subst_ctx_concat in Eq'.*)
-          exact Eq'.
-        }
-        rewrite <- Eq'.
-        (* Now we would like to swap the order of the two substitutions in the goal,
-           but that's not the same, because
-           (subst_ctx x y (subst_ctx x' x ...)) == (subst_ctx x' y)
-        *)
-        admit.
-
-(* notin: either use x # (subst x x' ...), or use x' # ...  *)
-      }
-
-(*
-  + (* case ty_hyp *)
-    introv WfT Ty IH Eq Ok Biy. subst.
-    apply ty_hyp.
-    - apply* subst_wf_typ.
-    - intros G' Se Gb.
-      rewrite subst_ctx_concat in *.
-      (*
-In IH, we must set x0:=x, y0:=y 
-in order to get (subst_trm x y t) (subst_typ x y T) in the conclusion.
-
-     
-         so the conclusion of the IH has no x in the env
-         
-        G' might contain an arbitary type for x, completely unrelated to S
-      rename that x into a fresh x'? --> x not in G' any more
-
-
-     what if we apply the undo lemma on the goal? wrong direction
-*)
-      assert (xG: x # (G1 & G2)) by apply closed_env_stuff.
-      lets P: (undo_subst_subenv Biy Se).
-      destruct P as [G1' [S' [G2' [? [Biy' Se']]]]]. subst.
-      rewrite <- subst_ctx_concat.
-      refine (IH _ Se' _ _ x y _ _ eq_refl (okadmit _) Biy').
-      assert (xG'': x # G1' & G2') by apply closed_env_stuff.
-      refine (undo_subst_good_bounds _ xG'' Gb).
-      apply (subst_binds_0 x y) in Biy'.
-      assert (xS': x \notin fv_typ S') by apply closed_env_stuff.
-      rewrite (subst_fresh_typ _ _ xS') in Biy'.
-      rewrite subst_ctx_concat in Biy'.
-      exact Biy'.
-      assert (E: exists G1'' S'' G2'', G'' = G1'' & x ~ S'' & G2'') by admit.
-      destruct E as [G1'' [S'' [G2'' E]]]. subst.
-
-      destruct (subenv_binds Se Biy') as [S' [Biy'' StS]].
-      assert (xG1': x \notin fv_ctx_types G1') by apply closed_env_stuff.
-      assert (xG2': x \notin fv_ctx_types G2') by apply closed_env_stuff.
-      (* should hold, because x is not in dom (G1' & G2'), and (G1' & G2') is closed *)
-      assert (xG': x # subst_ctx y x G1' & subst_ctx y x G2') by apply closed_env_stuff.
-      assert (xS': x \notin fv_typ S') by apply closed_env_stuff.
-      (* because in StS, S' is wf without any x being bound in the env *)
-      lets EqG1: (undo_subst_ctx y G1' xG1').
-      lets EqS:  (subst_typ_undo y S' xS').
-      lets EqG2: (undo_subst_ctx y G2' xG2').
-      lets Biy''': Biy''.
-      rewrite <- EqG1, <- EqG2 in Biy''', Gb. rewrite <- EqS in Biy'''.
-      lets P: (undo_subst_good_bounds Biy''' xG' Gb).
-      rewrite <- EqG1, <- EqG2.
-      rewrite <- subst_ctx_concat.
-      refine (IH _ _ P
-          (subst_ctx y x G1') x y _ (subst_ctx y x G2')
-          eq_refl (okadmit _) _); clear IH.
-      * admit. (*apply (subenv_undo_subst _ Biy'' Biy' Se' Se).*)
-      * rewrite <- subst_ctx_concat.
-        apply (subst_binds_0 _ _ Biy'').
-
-  + (* case ty_hyp *)
-    introv WfT Ty IH Eq Ok Biy. subst.
-    apply ty_hyp.
-    - apply* subst_wf_typ.
-    - intros G' Se Gb.
-      lets Biy': (subst_binds_0 x y Biy).
-      rewrite subst_ctx_concat in *.
-      destruct (subenv_concat_inv Se) as [G1' [G2' [? Se']]]. subst.
-      destruct (subenv_binds Se Biy') as [S' [Biy'' StS]].
-      assert (xG1': x \notin fv_ctx_types G1') by apply closed_env_stuff.
-      assert (xG2': x \notin fv_ctx_types G2') by apply closed_env_stuff.
-      (* should hold, because x is not in dom (G1' & G2'), and (G1' & G2') is closed *)
-      assert (xG': x # subst_ctx y x G1' & subst_ctx y x G2') by apply closed_env_stuff.
-      assert (xS': x \notin fv_typ S') by apply closed_env_stuff.
-      (* because in StS, S' is wf without any x being bound in the env *)
-      lets EqG1: (undo_subst_ctx y G1' xG1').
-      lets EqS:  (subst_typ_undo y S' xS').
-      lets EqG2: (undo_subst_ctx y G2' xG2').
-      lets Biy''': Biy''.
-      rewrite <- EqG1, <- EqG2 in Biy''', Gb. rewrite <- EqS in Biy'''.
-      admit. (*
-      lets P: (undo_subst_good_bounds Biy''' xG' Gb).
-      rewrite <- EqG1, <- EqG2.
-      rewrite <- subst_ctx_concat.
-      refine (IH _ _ P
-          (subst_ctx y x G1') x y _ (subst_ctx y x G2')
-          eq_refl (okadmit _) _); clear IH.
-      * admit. (*apply (subenv_undo_subst _ Biy'' Biy' Se' Se).*)
-      * rewrite <- subst_ctx_concat.
-        apply (subst_binds_0 _ _ Biy''). *)
-    *)
   + (* case ty_sbsm *)
     introv Ty IH St Eq Ok Biy. subst.
     lets St': (subst_subtyp St Ok Biy). apply ty_sbsm with (subst_typ x y T1); eauto.
@@ -5337,6 +4661,7 @@ in order to get (subst_trm x y t) (subst_typ x y T) in the conclusion.
     lets Hasnt: (subst_defs_hasnt x y d0).
     rewrite (subst_label_of_def x y d) in Hasnt.
     apply ty_defs_cons; fold subst_defs subst_def; eauto.
+  Grab Existential Variables. constructor. constructor. constructor. constructor.
 Qed.
 
 Lemma trm_subst_principle: forall G x y t S T,
@@ -5421,14 +4746,12 @@ Qed.
 (** ** Helpers *)
 
 Lemma invert_ty_var: forall G x T,
-  good_bounds G ->
   ty_trm G (trm_var (avar_f x)) T ->
-  exists T', binds x T' G /\ subtyp G T' T.
+  exists T', binds x T' G /\ subtyp okhyp G T' T.
 Proof.
-  introv Gb Ty. gen_eq t: (trm_var (avar_f x)). induction Ty; intro Eq; inversions Eq.
+  introv Ty. gen_eq t: (trm_var (avar_f x)). induction Ty; intro Eq; inversions Eq.
   - exists T. auto.
-  - apply* H1. apply subenv_refl.
-  - specialize (IHTy Gb eq_refl). destruct IHTy as [T0 [Bi St]].
+  - specialize (IHTy eq_refl). destruct IHTy as [T0 [Bi St]].
     exists T0. apply (conj Bi). apply (subtyp_trans St H).
 Qed.
 
@@ -5478,6 +4801,41 @@ Qed.
 
 
 (* ###################################################################### *)
+(** ** okhyp to nohyp *)
+
+Lemma anyhyp_to_nohyp:
+   (forall hm G T1 T2, subtyp hm G T1 T2 -> good_bounds G -> subtyp nohyp G T1 T2)
+/\ (forall hm G D1 D2, subdec hm G D1 D2 -> good_bounds G -> subdec nohyp G D1 D2).
+Proof.
+  apply subtyp_mutind.
+  + (* case subtyp_refl *) auto.
+  + (* case subtyp_top *) auto.
+  + (* case subtyp_bot *) auto.
+  + (* case subtyp_rcd *) auto.
+  + (* case subtyp_sel_l *)
+    introv Bix WfX Sb XHas St IH Gb. apply (subtyp_sel_l Bix WfX Sb XHas (IH Gb)).
+  + (* case subtyp_sel_r *)
+    introv Bix WfX Sb XHas St IH Gb. apply (subtyp_sel_r Bix WfX Sb XHas (IH Gb)).
+  + (* case subtyp_and *) auto.
+  + (* case subtyp_and_l *) auto.
+  + (* case subtyp_and_r *) auto.
+  + (* case subtyp_or *) auto.
+  + (* case subtyp_or_l *) auto.
+  + (* case subtyp_or_r *) auto.
+  + (* case subtyp_trans *) eauto.
+  + (* case subtyp_hyp *)
+    introv Bix XHas Sb WfX WfLo WfHi Gb.
+    unfold good_bounds, good_bounds_typ in Gb. specialize (Gb _ _ Bix).
+    destruct Gb as [_ Gb]. apply (Gb _ _ _ XHas).
+  + (* case subdec_typ *) auto.
+  + (* case subdec_mtd *) auto.
+Qed.
+
+Definition subtyp_to_nohyp := proj1 anyhyp_to_nohyp.
+Definition subdec_to_nohyp := proj2 anyhyp_to_nohyp.
+
+
+(* ###################################################################### *)
 (** ** Progress *)
 
 Lemma progress_proof:
@@ -5504,9 +4862,10 @@ Proof.
         destruct IHarg as [s' [e' IHarg]]. do 2 eexists. apply (red_call2 x m IHarg).
       * (* arg is a var *)
         destruct IHarg as [y [o [Eq Bisy]]]. subst.
-        apply (invert_ty_var (wf_sto_to_good_bounds Wfs)) in Ty1.
+        apply invert_ty_var in Ty1.
         destruct Ty1 as [T' [BiG StT]].
-        lets P: (swap_sub_and_typ_has StT THas). destruct P as [D1 [T'Has Sd]].
+        lets P: (subtyp_to_memberwise (subtyp_to_nohyp StT (wf_sto_to_good_bounds Wfs))).
+        destruct P as [P _]. specialize (P _ THas). destruct P as [D1 [T'Has Sd]].
         apply invert_subdec_mtd_sync_left in Sd. destruct Sd as [U' [V' [Eq [StU StV]]]].
         subst.
         lets P: (typ_has_to_defs_has Wfs T'Has Bis BiG).
@@ -5519,10 +4878,6 @@ Proof.
     left. pick_fresh x.
     exists (open_trm x u) (s & x ~ (open_defs x ds)).
     apply* red_new.
-  + (* case ty_hyp *)
-    introv WfT Ty IH Wfs.
-    lets Gb: (wf_sto_to_good_bounds Wfs).
-    apply* IH. apply subenv_refl.
   + (* case ty_sbsm *)
     introv Ty IH St Wf. apply (IH s Wf).
 Qed.
@@ -5618,7 +4973,6 @@ Proof.
 Qed.
 
 Lemma invert_ty_new: forall G ds u U,
-  good_bounds G ->
   ty_trm G (trm_new ds u) U ->
   exists L T,
      (forall x, x \notin L ->
@@ -5627,10 +4981,9 @@ Lemma invert_ty_new: forall G ds u U,
         ty_trm (G & x ~ open_typ x T) (open_trm x u) U)
   /\ (wf_typ G U).
 Proof.
-  introv Gb Ty. gen_eq t: (trm_new ds u). induction Ty; intro Eq; inversions Eq.
+  introv Ty. gen_eq t: (trm_new ds u). induction Ty; intro Eq; inversions Eq.
   - eauto.
-  - apply* H1. apply subenv_refl.
-  - specialize (IHTy Gb eq_refl).
+  - specialize (IHTy eq_refl).
     destruct IHTy as [L [T0 [Tyds [Tyu Wf]]]].
     subst. exists L T0. repeat split.
     * apply Tyds.
@@ -5639,18 +4992,16 @@ Proof.
 Qed.
 
 Lemma invert_ty_call: forall G t m V2 u,
-  good_bounds G ->
   ty_trm G (trm_call t m u) V2 ->
   exists T U V1,
     ty_trm G t T /\
     typ_has G T (dec_mtd m U V1) /\
     ty_trm G u U /\
-    subtyp G V1 V2.
+    subtyp okhyp G V1 V2.
 Proof.
-  introv Gb Ty. gen_eq t0: (trm_call t m u). induction Ty; intro Eq; inversions Eq.
+  introv Ty. gen_eq t0: (trm_call t m u). induction Ty; intro Eq; inversions Eq.
   - do 3 eexists. eauto.
-  - apply (H1 _ (@subenv_refl _) Gb Gb eq_refl).
-  - specialize (IHTy Gb eq_refl). destruct IHTy as [T [U [V [Tyt [THas [Tyu St]]]]]].
+  - specialize (IHTy eq_refl). destruct IHTy as [T [U [V [Tyt [THas [Tyu St]]]]]].
     exists T U V. repeat split; auto. apply (subtyp_trans St H).
 Qed.
 
@@ -5713,11 +5064,12 @@ Proof.
     rename H into Bis, H0 into dsHas, T into U2, U into V2, V into V2'.
     exists (@empty typ). rewrite concat_empty_r. apply (conj Wf).
     lets Gb: (wf_sto_to_good_bounds Wf).
-    apply (invert_ty_call Gb) in TyCall.
+    apply invert_ty_call in TyCall.
     destruct TyCall as [T [U2'' [V2'' [Tyx [THas [Tyy StV]]]]]].
-    apply (invert_ty_var Gb) in Tyx. destruct Tyx as [T' [BiGx StT]].
-    apply (invert_ty_var Gb) in Tyy. destruct Tyy as [U2''' [BiGy StU2]].
-    lets P: (swap_sub_and_typ_has StT THas). destruct P as [D1 [T'Has Sd]].
+    apply invert_ty_var in Tyx. destruct Tyx as [T' [BiGx StT]].
+    apply invert_ty_var in Tyy. destruct Tyy as [U2''' [BiGy StU2]].
+    lets P: (subtyp_to_memberwise (subtyp_to_nohyp StT (wf_sto_to_good_bounds Wf))).
+    destruct P as [P _]. specialize (P _ THas). destruct P as [D1 [T'Has Sd]].
     apply invert_subdec_mtd_sync_left in Sd. destruct Sd as [U1 [V1 [Eq [StU1 StV']]]].
     subst D1.
     lets P: (typ_has_to_defs_has Wf T'Has Bis BiGx). destruct P as [d [dsHas' Tyd]].
@@ -5728,7 +5080,7 @@ Proof.
     }
     inversions Eq. clear dsHas'.
     rename U2''' into U1.
-    lets StU: (subtyp_trans StU2 StU1).
+    lets StU: (subtyp_trans StU2 (subtyp_to_okhyp StU1)).
     pick_fresh y'.
     assert (y'L: y' \notin L) by auto.
     specialize (Tybody y' y'L).
@@ -5744,8 +5096,9 @@ Proof.
       apply (weaken_good_bounds_typ_end Oky' GbU2).
     }
     *)
+    lets StU0: (subtyp_to_nohyp StU (wf_sto_to_good_bounds Wf)). clear StU.
     assert (Oky': ok (G & y' ~ U1)) by auto.
-    apply (weaken_subtyp_end Oky') in StU.
+    lets StU: (weaken_subtyp_end Oky' StU0).
     destruct (ctx_binds_to_sto_binds Wf BiGy) as [dsy [Bisy Tydsy]].
     lets SbU1: (defs_have_stable_typ Tydsy).
     lets Tybody': (narrow_ty_end Tybody Oky' SbU1 StU).
@@ -5756,11 +5109,11 @@ Proof.
     rewrite <- (@subst_intro_trm y' y body y'body) in P.
     apply (ty_sbsm P).
     assert (EqV2: (subst_typ y' y V2) = V2). { refine (@subst_fresh_typ y' y _ _). auto. }
-    rewrite EqV2. apply (subtyp_trans StV' StV).
+    rewrite EqV2. apply (subtyp_trans (subtyp_to_okhyp StV') StV).
   + (* red_new *)
     introv Wf Ty.
     lets Gb: (wf_sto_to_good_bounds Wf).
-    apply (invert_ty_new Gb) in Ty.
+    apply invert_ty_new in Ty.
     destruct Ty as [L [Tds [Tyds [Tyt WfT]]]].
     exists (x ~ (open_typ x Tds)).
     assert (xG: x # G) by apply* sto_unbound_to_ctx_unbound.
@@ -5781,7 +5134,7 @@ Proof.
   + (* red_call1 *)
     intros G Tr2 Wf TyCall.
     lets Gb: (wf_sto_to_good_bounds Wf).
-    apply (invert_ty_call Gb) in TyCall.
+    apply invert_ty_call in TyCall.
     destruct TyCall as [To2 [Ta [Tr1 [Tyo [Has [Tya Str]]]]]].
     specialize (IHRed _ _ Wf Tyo). destruct IHRed as [G' [Wf' Tyo']].
     exists G'. apply (conj Wf').
@@ -5795,7 +5148,7 @@ Proof.
   + (* red_call2 *)
     intros G Tr2 Wf TyCall.
     lets Gb: (wf_sto_to_good_bounds Wf).
-    apply (invert_ty_call Gb) in TyCall.
+    apply invert_ty_call in TyCall.
     destruct TyCall as [To2 [Ta [Tr1 [Tyo [Has [Tya Str]]]]]].
     specialize (IHRed _ _ Wf Tya). destruct IHRed as [G' [Wf' Tya']].
     lets Ok': (wf_sto_to_ok_G Wf').
